proof/correctness/avx2/common/NTT_avx2_poly.ec
@@ -360,6 +360,51 @@ lemma poly_invntt_avx2_corr _r :
 proof.
 conseq poly_invntt_avx2_eq (invntt_avx_spec (lift_array256 _r)).
 move => &1 [<- H]. exists (lift_array256 arg{1}) => />. rewrite lift_nttpack perm_ntt_nttpackE //.
-move => &1 &2 [<- H] -> /#. 
+move => &1 &2 [<- H] -> /#.
 qed.
+
+(* variant-independent register shuffles (relocated from the per-variant NTT_avx2) *)
+abbrev shuffle8_idx = Array32.of_list witness
+  [0; 1; 2; 3; 4; 5; 6; 7; 16; 17; 18; 19; 20; 21; 22; 23;
+   8; 9; 10; 11; 12; 13; 14; 15; 24; 25; 26; 27; 28; 29; 30; 31].
+
+abbrev shuffle4_idx = Array32.of_list witness
+  [0; 1; 2; 3; 16; 17; 18; 19; 8; 9; 10; 11; 24; 25; 26; 27;
+   4; 5; 6; 7; 20; 21; 22; 23; 12; 13; 14; 15; 28; 29; 30; 31].
+
+abbrev shuffle2_idx = Array32.of_list witness
+  [0; 1; 16; 17; 4; 5; 20; 21; 8; 9; 24; 25; 12; 13; 28; 29;
+   2; 3; 18; 19; 6; 7; 22; 23; 10; 11; 26; 27; 14; 15; 30; 31].
+
+abbrev shuffle1_idx = Array32.of_list witness
+  [0; 16; 2; 18; 4; 20; 6; 22; 8; 24; 10; 26; 12; 28; 14; 30;
+   1; 17; 3; 19; 5; 21; 7; 23; 9; 25; 11; 27; 13; 29; 15; 31].
+
+op shuf8 (a b: 'a Array16.t) : ('a Array16.t * 'a Array16.t) =
+  let c = Array32.init (fun i => if 16 <= i then b.[i %% 16] else a.[i]) in
+  let cr = Array32.init (fun i => c.[shuffle8_idx.[i]]) in
+  let ar = Array16.init (fun i => cr.[i]) in
+  let br = Array16.init (fun i => cr.[i + 16]) in
+  (ar, br).
+
+op shuf4 (a b: 'a Array16.t) : ('a Array16.t * 'a Array16.t) =
+  let c = Array32.init (fun i => if 16 <= i then b.[i %% 16] else a.[i]) in
+  let cr = Array32.init (fun i => c.[shuffle4_idx.[i]]) in
+  let ar = Array16.init (fun i => cr.[i]) in
+  let br = Array16.init (fun i => cr.[i + 16]) in
+  (ar, br).
+
+op shuf2 (a b: 'a Array16.t) : ('a Array16.t * 'a Array16.t) =
+  let c = Array32.init (fun i => if 16 <= i then b.[i %% 16] else a.[i]) in
+  let cr = Array32.init (fun i => c.[shuffle2_idx.[i]]) in
+  let ar = Array16.init (fun i => cr.[i]) in
+  let br = Array16.init (fun i => cr.[i + 16]) in
+  (ar, br).
+
+op shuf1 (a b: 'a Array16.t) : ('a Array16.t * 'a Array16.t) =
+  let c = Array32.init (fun i => if 16 <= i then b.[i %% 16] else a.[i]) in
+  let cr = Array32.init (fun i => c.[shuffle1_idx.[i]]) in
+  let ar = Array16.init (fun i => cr.[i]) in
+  let br = Array16.init (fun i => cr.[i + 16]) in
+  (ar, br).
 
