proof/correctness/avx2/1024/MLKEM_Poly_avx2_circuit_1024.ec
@@ -1,0 +1,144 @@
+require import AllCore List Int IntDiv CoreMap Real Number Ring StdOrder BitEncoding.
+
+from Jasmin require import JModel.
+from JazzEC require import Array400 Array384 Array256 Array160 Array128 Array64 Array32 Array16 Array8 Array4 Array2.
+from JazzEC require import WArray512 WArray128 WArray384 WArray32 WArray16.
+from JazzEC require import Jkem_avx2.
+
+require import AVX2_Ops W16extra.
+require import Fq NTT_Fq MLKEMFCLib MLKEM_W16_Rep MLKEM1024_prelude.
+require import Fq_avx2 NTT_avx2 NTT_avx2_poly AVX2_Ops MLKEMFCLib.
+require import MLKEM_Poly_avx2.
+require import Mlkem_bindings.
+require import Circuit_semantics Circuit_sem_1024.
+from Spec require import GFq Rq Serialization VecMat Sampling EncDecCorrectness Correctness.
+
+import BitChunking BS2Int.
+import Fq.
+import GFq Rq Serialization VecMat.
+import Zq ZModP.
+import Fq_avx2 NTT_Avx2.
+import MLKEMFCLib1024.
+import MLKEM_PolyAVX.
+import W12.
+
+abbrev encode5 (a : ipoly) : W8.t Array160.t = Array160.of_list W8.zero (ByteEncode 5 (to_list a)).
+
+
+lemma poly_decompress_ll : islossless Jkem_avx2.M._i_poly_decompress.
+ proc; inline *;wp. cfold 5; unroll for ^while;auto. 
+qed.
+
+lemma poly_decompress_corr_h (_a : W8.t Array160.t): 
+    hoare [Jkem_avx2.M._i_poly_decompress  :
+              arg.`2 = _a
+              ==>
+             lift_array256 res = decompress_poly 5 (decode5 _a) /\
+             pos_bound256_cxq res 0 256 1 ].
+proc; inline *.
+proc change 1: { q <- sliceget16_16_256 jqx16 0;} ; 1: by auto.
+proc change 2: { shufbidx <- sliceget32_8_256 pd_jshufbidx 0; }; 1: by auto.
+proc change 3: { mask <- sliceget16_16_256 pd_mask_s 0;} ; 1: by auto.
+proc change 4: { shift <- sliceget16_16_256 pd_shift_s 0; } ; 1: by auto.
+proc change ^while.1 : { t <- zeroextu128 (sliceget160_8_64 a ((10*i)*8)); };1: by auto => /#.
+proc change ^while.10 : { rp <- sliceset256_16_256 rp (i*256) f; };1: by auto => /#.
+proc change ^while.2: { ti <- sliceget160_8_16 a ((10*i+8)*8); };1: by auto => /#.
+
+cfold 5.
+unroll for ^while.
+cfold ^i<-.
+wp -2.
+
+conseq (: _ ==> rp = init_256_16 (fun i =>
+     decompress5_circuit (W5.init (fun (j : int) => _a.[(i*5 + j) %/ 8].[(i*5 + j) %% 8])))); last  by circuit.
+
+      
+(* We start with some boilerplate *)
+move => &hr [#]/= <- rr /= ->.
+
+split.
++ rewrite tP => i ib.
+  rewrite /init_256_16 !mapiE 1,2:/# /= -get_to_list /= initiE 1:/# /=.
+  rewrite /decompress5_circuit decompress5_circuit_sem //.
+
+rewrite /pos_bound256_cxq qE /= => k kb. 
+rewrite /init_256_16 initiE 1:/# /=.
+by apply decompress5_circuit_rng.
+qed.
+
+(********** END BDEP PROOF OF DECOMPRESS **************)
+
+lemma poly_decompress_corr (_a : W8.t Array160.t): 
+    phoare [Jkem_avx2.M._i_poly_decompress  :
+              arg.`2 = _a
+              ==>
+             lift_array256 res = decompress_poly 5 (decode5 _a) /\
+             pos_bound256_cxq res 0 256 1 ] = 1%r
+  by conseq poly_decompress_ll (poly_decompress_corr_h _a).
+
+lemma i_poly_compress_corr_ll : islossless Jkem_avx2.M._i_poly_compress.
+proof.
+proc; inline *.
+cfold 13.
+do 2!(unroll for ^while).
+auto.
+qed.
+
+lemma i_poly_compress_corr_h _aw  : 
+    hoare [Jkem_avx2.M._i_poly_compress  :
+             pos_bound256_cxq a 0 256 2 /\
+             a = _aw
+              ==>
+             res.`1 = encode5 (compress_poly 5 (lift_array256 _aw)) 
+             ].
+proof.
+proc; inline *.
+proc change 2: { qx16 <- sliceget16_16_256 jqx16 0;} ; 1: by auto.
+proc change ^while.1: { r <- sliceget256_16_256 rp0 (i0*256);} ;1: by auto => /#.
+proc change ^while.9: { rp0 <- sliceset256_16_256 rp0 (i0*256) r; } ;1: by auto => /#.
+proc change 6: { v <- sliceget16_16_256 jvx16 0; }; 1: by auto.
+proc change 12: { shufbidx <- sliceget32_8_256 pc_shufbidx_s 0; }; 1: by auto.
+proc change ^while{2}.1: { f0 <- sliceget256_16_256 a (2*i*256);} ;1: by auto => /#.
+proc change ^while{2}.2: { f1 <- sliceget256_16_256 a ((2*i+1)*256); };1: by auto => /#.
+proc change ^while{2}.18 : { rp <- sliceset160_8_128 rp  (20*i*8) t0;};1: by auto => /#.
+proc change ^while{2}.19 : { rp <- sliceset160_8_32 rp  ((20*i+16)*8) (truncateu32 t1);}.
++ by auto => /> &m; move: (truncateu32 t1{m}) => ? /#.
+
+cfold 13.
+do 2!(unroll for ^while).
+cfold ^i0<-.
+wp -3.
+
+conseq (: a = _aw /\
+   Array256.all (fun bv => W16.zero \sle bv /\ bv \slt (of_int (2 * 3329))) a
+   ==> rp = init_160_8 (fun i =>
+     W8.init (fun j =>
+       (compress5_circuit _aw.[(i*8+j) %/ 5]).[(i*8+j) %% 5]))); last by circuit.
+        
+       
+(* BDEP pre conseq *)
++ move => &hr />; rewrite /pos_bound256_cxq qE /= /(\sle) /(\slt) allP /=  => Hb i ib /=.
+  rewrite /(to_sint W16.zero) /= /(W16.smod 0) /=.
+  rewrite /(to_sint (W16.of_int 6658)) /= /(W16.smod 6658) /= /#.
+  
+(* BDEP post conseq *)
+
+(* We start with some boilerplate *)
+move => &hr [#]/= H0 <- rr ->; rewrite /= /init_128_8 tP => i ib.
+rewrite wordP => k kb; rewrite !initiE 1..3:/# /=.
+rewrite encode_compress_bits //=.
+by apply compress5_circuit_sem.
+qed.
+
+
+
+(********** END BDEP PROOF OF COMPRESS **************)
+
+lemma i_poly_compress_corr _aw  : 
+    phoare [Jkem_avx2.M._i_poly_compress  :
+             pos_bound256_cxq a 0 256 2 /\
+             a = _aw
+              ==>
+             res.`1 = encode5 (compress_poly 5 (lift_array256 _aw)) 
+             ] = 1%r
+ by conseq i_poly_compress_corr_ll (i_poly_compress_corr_h _aw).
