proof/correctness/avx2/1024/circuit_sem_1024.ec
@@ -1,0 +1,512 @@
+require import AllCore List Int IntDiv CoreMap Real Number Ring StdOrder BitEncoding.
+
+from Jasmin require import JModel.
+from JazzEC require import Array256 Array128 Array64 Array32 Array16 Array8 Array4 Array2.
+from JazzEC require import Array768 Array960 Array1152 Array1024 Array1408 Array1536 Array160 Array2304.
+from JazzEC require import Jkem_avx2.
+
+require import AVX2_Ops W16extra.
+require import Fq NTT_Fq MLKEMFCLib MLKEM_W16_Rep MLKEM1024_prelude.
+require import Mlkem_bindings.
+require import Circuit_semantics.
+from Spec require import GFq Rq Serialization VecMat Sampling EncDecCorrectness Correctness.
+
+import BitChunking BS2Int.
+import Fq.
+import GFq Rq Serialization VecMat.
+import Zq ZModP IntOrder BitReverse.
+import PolyVec PolyMat.
+import MLKEMFCLib1024.
+import W12.
+
+abbrev decode11_vec (a : W8.t Array1408.t) : ipolyvec = IPVec.of_list 0 (ByteDecode 11 (to_list a)).
+abbrev decode5 (a : W8.t Array160.t) : ipoly = Array256.of_list 0 (ByteDecode 5 (to_list a)).
+
+
+lemma to_bytes_circuit_sem_polyvec (p : W16.t Array1024.t) (i k : int) :
+    p.[(i * 8 + k) %/ 12] \ult W16.of_int (2*3329) =>
+        0 <= i < 1536 =>
+        0 <= k < 8 =>
+((tobytes_circuit p.[(i * 8 + k) %/ 12]).[(i * 8 + k) %% 12])%W12 =
+(ByteEncode 12 (to_list (map asint (lift_array1024 p)))).[i].[k].
+proof.
+rewrite /(\ult) /=  => bd Hi Hk.
+rewrite /ByteEncode /BitsToBytes (nth_map []).
++ rewrite size_chunk // (EclibExtra.size_flatten' 12);1: smt(mapP BS2Int.size_int2bs).
+  by rewrite size_map size_to_list /=.
+rewrite JWordList.nth_chunk 1,2:/#.
++ rewrite (EclibExtra.size_flatten' 12);1: smt(mapP BS2Int.size_int2bs).
+  by rewrite size_map size_to_list /=; smt(kvec_val).
+rewrite get_bits2w // nth_take 1,2:/# nth_drop 1,2:/#.
+rewrite (nth_flatten false 12);1:by  rewrite allP;smt(mapP BS2Int.size_int2bs).
+rewrite (nth_map witness);1: rewrite size_to_list /#.
+rewrite get_to_list mapiE 1:/# /lift_array256 mapiE 1:/# /= incoeffK.
+rewrite /tobytes_circuit /(\ult) /=.
+case (to_uint p.[(i * 8 + k) %/ 12] < 3329) => ?.
++ rewrite /truncateu12 /of_int get_bits2w 1:/# /= modz_small;1:smt(W16.to_uint_cmp).
+  rewrite qE (modz_small _ 3329); 1,2: by rewrite /to_sint /smod /=;smt(W16.to_uint_cmp pow2_16).
+have -> : (W16_sub p.[(i * 8 + k) %/ 12] (W16.of_int 3329))=
+          W16.of_int (to_sint p.[(8 * i + k) %/ 12] %% q); last first.
++ rewrite /truncateu12 of_uintK  /= modz_small;1:smt(W16.to_uint_cmp).
+  rewrite /of_int get_bits2w 1:/# /= /#.
+rewrite /W16_sub /= to_uint_eq of_uintK modz_small;1:smt(W16.to_uint_cmp).
+rewrite to_uintB /=;1: rewrite /(\ule) /= /#.
+rewrite /to_sint /smod /= /#.
+qed.
+
+
+op decompress11_circuit(c : W11.t) : W16.t = 
+  truncateu16 (srl_32 (((zeroextu11_32 c) * W32.of_int 3329) + W32.of_int 1024) (W32.of_int 11)).
+
+
+lemma pow2_11 : 2^11 = 2048 by auto.
+
+
+lemma decompress11_circuit_sem (a : W8.t Array1408.t) (i : int) :
+        0 <= i < 1024 =>
+        incoeff (to_sint (decompress11_circuit (W11.init (fun (j : int) => a.[(i*11 + j) %/ 8].[(i*11 + j) %% 8])))) =
+Decompress 11 (decode11_vec a).[i].
+proof.
+move => ib. 
+rewrite -decompress_alt_decompress // /decompress_alt;congr.
+rewrite get_of_list; 1: by smt(kvec_val).
+rewrite /ByteDecode (nth_map []);
+ 1: by rewrite size_chunk // size_BytesToBits size_to_list /#.
+rewrite /decompress11_circuit /to_sint to_uint_truncateu16 /srl_32 to_uint_shr //=.
+rewrite to_uintD_small /=.
++ rewrite to_uintM_small /zeroextu11_32 of_uintK /= modz_small /=;by smt(W11.to_uint_cmp pow2_11).  
+rewrite to_uintM_small /=; 1: by rewrite /zeroextu11_32 of_uintK //= modz_small /=;by smt(W11.to_uint_cmp pow2_11).
+rewrite /smod ifF /=; 1: by rewrite /zeroextu5_32 of_uintK /= modz_small /=;by smt(W11.to_uint_cmp pow2_11).
+rewrite /zeroextu11_32 of_uintK /= modz_small /=;1: by smt(W11.to_uint_cmp pow2_11).
+rewrite modz_small /=;1: by smt(W11.to_uint_cmp pow2_11).
+rewrite /to_uint;congr;congr;congr;congr;last by smt().
+congr;apply (eq_from_nth false).
++ by rewrite size_w2bits size_nth_chunk // size_BytesToBits size_to_list /#.
+move => k; rewrite size_w2bits => kb.
+rewrite get_w2bits initiE 1:/# /=  JWordList.nth_chunk 1,2:/#.
++ by rewrite size_BytesToBits size_to_list /#.
+rewrite /BytesToBits nth_take 1,2:/# nth_drop 1,2:/#.
+rewrite (nth_flatten false 8); 1:by  rewrite allP; smt(mapP W8.size_w2bits  size_map).
+rewrite (nth_map witness);1: by rewrite size_to_list /= /#.
+rewrite (nth_map witness);1: by rewrite size_iota /= /#.
+by rewrite nth_iota /#.
+qed.
+
+lemma decompress11_circuit_rng  (a : W8.t Array1408.t) (i : int) :
+     0 <= i < 1024 =>   
+     0 <= to_sint (decompress11_circuit (W11.init (fun (j : int) => a.[(i*11 + j) %/ 8].[(i*11 + j) %% 8]))) < 3329.
+proof.
+move => ib.
+rewrite /decompress11_circuit /to_sint to_uint_truncateu16 /srl_32 to_uint_shr //=.
+rewrite to_uintD_small /=.
++ rewrite to_uintM_small /zeroextu11_32 of_uintK /= modz_small /=;by smt(W11.to_uint_cmp pow2_11).  
+rewrite to_uintM_small /=; 1: by rewrite /zeroextu5_32 of_uintK //= modz_small /=;by smt(W11.to_uint_cmp pow2_11).
+rewrite /smod ifF /=; 1: by rewrite /zeroextu5_32 of_uintK /= modz_small /=;by smt(W11.to_uint_cmp pow2_11).
+rewrite /zeroextu11_32 of_uintK /= modz_small /=;1: by smt(W11.to_uint_cmp pow2_11).
+rewrite modz_small /=; by smt(W11.to_uint_cmp pow2_11).
+qed.
+
+lemma frombytes_circuit_sem (a : W8.t Array1536.t) (i : int) :
+        0 <= i < 1024 =>
+        incoeff (to_sint (frombytes_circuit
+             (W12.init (fun (j : int) => a.[(i * 12 + j) %/ 8].[(i * 12 + j) %% 8])))) =
+        incoeff (IPVec.of_list 0 (ByteDecode 12 (to_list a))).[i].
+proof.
+move => ib.
+rewrite get_of_list; 1: by smt(kvec_val).
+rewrite /ByteDecode (nth_map []);
+ 1: by rewrite size_chunk // size_BytesToBits size_to_list /#.
+rewrite /frombytes_circuit /to_sint /zeroextu16 of_uintK /= modz_small /=; 1: by have :=  W12.to_uint_cmp => /= /#.
+rewrite /BytesToBits JWordList.nth_chunk 1,2:/#.
+rewrite (EclibExtra.size_flatten' 8);1,2:smt(mapP W8.size_w2bits Array1536.size_to_list size_map).
+congr.
+rewrite /smod /=.
+rewrite ifF; 1: by have :=  W12.to_uint_cmp => /= /#.
+rewrite /to_uint;congr;apply (eq_from_nth false).
++ rewrite W12.size_w2bits size_take 1:/# size_drop 1:/#.
+  rewrite (EclibExtra.size_flatten' 8);1,2:smt(mapP W8.size_w2bits Array1536.size_to_list size_map).
+move => k; rewrite W12.size_w2bits => kb.
+rewrite W12.get_w2bits W12.initiE 1:/# /=.
+rewrite nth_take 1,2:/# nth_drop 1,2:/#.
+rewrite (nth_flatten false 8);1: by rewrite allP => x;rewrite mapP => Hx;elim Hx;smt(W8.size_w2bits).
+rewrite (nth_map witness);1: by rewrite size_to_list /= /#.
+rewrite get_to_list get_w2bits /#.
+qed.
+
+lemma frombytes_circuit_rng  (a : W8.t Array1536.t) (i : int) :
+     0 <= to_sint (frombytes_circuit
+             (W12.init (fun (j : int) => a.[(i * 12 + j) %/ 8].[(i * 12 + j) %% 8])))< 4096.
+proof.
+rewrite /frombytes_circuit.
+rewrite  /to_sint  /to_sint /zeroextu16 of_uintK /= modz_small /=; 1: by have :=  W12.to_uint_cmp => /= /#.
+rewrite /smod /=.
+have :=  W12.to_uint_cmp => /=/#.
+qed.
+
+
+op compress5_circuit(a : W16.t) : W5.t = 
+   if (a \ult W16.of_int 3329) then  
+   truncateu32_5 (srl_32 ((sll_32 (zeroextu32 a) (W32.of_int 5) + W32.of_int 1664) * W32.of_int 40318) (W32.of_int 27))
+   else 
+   truncateu32_5 (srl_32 ((sll_32 (zeroextu32 (W16_sub a (W16.of_int 3329))) (W32.of_int 5) + W32.of_int 1664) * W32.of_int 40318) (W32.of_int 27)).  
+
+ 
+
+lemma compress5_circuit_sem (p : W16.t Array256.t) (i k : int) :
+        0 <= i < 160 =>
+        0 <= k < 8 =>
+     pos_bound256_cxq p 0 256 2 =>
+(compress5_circuit p.[(i * 8 + k) %/ 5]).[(i * 8 + k) %% 5] =
+(Compress 5 (incoeff (to_sint p.[(8 * i + k) %/ 5])) %/ 2 ^ ((8 * i + k) %% 5) %% 2 <> 0).
+proof.
+move => Hi Hk /=; rewrite /compress5_circuit  /pos_bound256_cxq qE /= => H00.
+rewrite ultE /= get_to_uint.
+have ->/= : (0 <= (i * 8 + k) %% 5 < 5) by smt().
+case (to_uint p.[(i * 8 + k) %/ 5] < 3329) => /= *. 
++ rewrite -Fq.Fq1024.compress_impl5 //=; 1: by rewrite /bpos16 qE /= /to_sint /smod /=;smt(W16.to_uint_cmp).  
+  congr;congr;congr;congr;congr;congr; 2: by smt().
+  rewrite /truncateu32_4 of_uintK /=. 
+  by rewrite /srl_32 /sll_32 /(`<<`) /(`>>`) /= /#.
+
+  
+have -> : (incoeff (to_sint p.[(8 * i + k) %/ 5])) = (incoeff (to_sint (W16_sub p.[(8 * i + k) %/ 5] (W16.of_int 3329)))); last first.
++ rewrite -Fq.Fq1024.compress_impl5 //=.
+  rewrite to_sintB_small /=;1: by rewrite  /(to_sint (W16.of_int 3329)) /= /smod /=;smt(size_map size_iota).
+  rewrite  /smod /= qE; have := H00 ((8 * i + k) %/ 5) _; 1: by smt().
+  move => Hb; have E: to_sint (W16.of_int 3329) = 3329 by rewrite /to_sint /smod /=.
+  by rewrite E; smt(W16.to_uint_cmp pow2_16 W16.to_sintE).
+  rewrite /truncateu32_4 of_uintK /=.
+  by rewrite /srl_32 /sll_32 /(`<<`) /(`>>`) /= /#.
+
+rewrite -eq_incoeff.
+rewrite to_sintB_small /=;1: by rewrite  /(to_sint (W16.of_int 3329)) /smod /=;smt(size_map size_iota). 
+   by rewrite  /(to_sint (W16.of_int 3329))  /smod /=; smt(size_map size_iota W16.to_uint_cmp).
+qed.
+
+op decompress5_circuit(c : W5.t) : W16.t =
+  truncateu16 (srl_32 (((zeroextu5_32 c) * W32.of_int 3329) + W32.of_int 16) (W32.of_int 5)).
+
+lemma decompress5_circuit_sem (a : W8.t Array160.t) (i : int) :
+        0 <= i < 256 =>
+        incoeff (to_sint (decompress5_circuit (W5.init (fun (j : int) => a.[(i*5 + j) %/ 8].[(i*5 + j) %% 8])))) =
+Decompress 5 (decode5 a).[i].
+proof.
+move => ib. 
+rewrite -decompress_alt_decompress // /decompress_alt;congr.
+rewrite /decode5 /= get_of_list // /ByteDecode (nth_map []);
+ 1: by rewrite size_chunk // size_BytesToBits size_to_list /#.
+rewrite /decompress5_circuit /to_sint to_uint_truncateu16 /srl_32 to_uint_shr //=.
+rewrite to_uintD_small /=.
++ rewrite to_uintM_small /zeroextu5_32 of_uintK /= modz_small /=;by smt(W5.to_uint_cmp pow2_5).  
+rewrite to_uintM_small /=; 1: by rewrite /zeroextu5_32 of_uintK //= modz_small /=;by smt(W5.to_uint_cmp pow2_5).
+rewrite /smod ifF /=; 1: by rewrite /zeroextu5_32 of_uintK /= modz_small /=;by smt(W5.to_uint_cmp pow2_5).
+rewrite /zeroextu5_32 of_uintK /= modz_small /=;1: by smt(W5.to_uint_cmp pow2_5).
+rewrite modz_small /=;1: by smt(W5.to_uint_cmp pow2_5).
+rewrite /to_uint;congr;congr;congr;congr;last by smt().
+congr;apply (eq_from_nth false).
++ by rewrite size_w2bits size_nth_chunk // size_BytesToBits size_to_list /#.
+move => k; rewrite size_w2bits => kb.
+rewrite get_w2bits initiE 1:/# /=  JWordList.nth_chunk 1,2:/#.
++ by rewrite size_BytesToBits size_to_list /#.
+rewrite /BytesToBits nth_take 1,2:/# nth_drop 1,2:/#.
+rewrite (nth_flatten false 8); 1:by  rewrite allP; smt(mapP W8.size_w2bits Array32.size_to_list size_map).
+rewrite (nth_map witness);1: by rewrite size_to_list /= /#.
+rewrite (nth_map witness);1: by rewrite size_iota /= /#.
+by rewrite nth_iota /#.
+qed.
+
+lemma decompress5_circuit_rng  (a : W8.t Array160.t) (i : int) :
+     0 <= i < 256 =>   
+     0 <= to_sint (decompress5_circuit (W5.init (fun (j : int) => a.[(i*5 + j) %/ 8].[(i*5 + j) %% 8]))) < 3329.
+proof.
+move => ib.
+rewrite /decompress5_circuit /to_sint to_uint_truncateu16 /srl_32 to_uint_shr //=.
+rewrite to_uintD_small /=.
++ rewrite to_uintM_small /zeroextu5_32 of_uintK /= modz_small /=;by smt(W5.to_uint_cmp pow2_5).  
+rewrite to_uintM_small /=; 1: by rewrite /zeroextu5_32 of_uintK //= modz_small /=;by smt(W5.to_uint_cmp pow2_5).
+rewrite /smod ifF /=; 1: by rewrite /zeroextu5_32 of_uintK /= modz_small /=;by smt(W5.to_uint_cmp pow2_5).
+rewrite /zeroextu5_32 of_uintK /= modz_small /=;1: by smt(W5.to_uint_cmp pow2_5).
+rewrite modz_small /=; by smt(W5.to_uint_cmp pow2_5).
+qed.
+
+op compress11_circuit(a : W16.t) : W11.t = 
+   if (a \ult W16.of_int 3329) then  
+   truncate64_11 (srl_64 ((sll_64 (zeroextu64 a) (W64.of_int 11) + W64.of_int 1664) * W64.of_int 645084) (W64.of_int 31))
+   else 
+   truncate64_11 (srl_64 ((sll_64 (zeroextu64 (W16_sub a (W16.of_int 3329))) (W64.of_int 11) + W64.of_int 1664) * W64.of_int 645084) (W64.of_int 31)).
+
+   
+import BitEncoding BS2Int BitChunking.
+from JazzEC require import Array8.
+
+
+lemma compress11_circuit_sem (p : W16.t Array1024.t) (i k : int) :
+        0 <= i < 1408 =>
+        0 <= k < 8 =>
+     pos_bound1024_cxq p 0 1024 2 =>
+(compress11_circuit p.[(i * 8 + k) %/ 11]).[(i * 8 + k) %% 11] =
+(Compress 11 (incoeff (to_sint p.[(8 * i + k) %/ 11])) %/ 2 ^ ((8 * i + k) %% 11) %% 2 <> 0).
+proof.
+move => Hi Hk /=; rewrite /compress11_circuit  /pos_bound1024_cxq qE /= => H00.
+rewrite ultE /= get_to_uint.
+have ->/= : (0 <= (i * 8 + k) %% 11 < 11) by smt().
+case (to_uint p.[(i * 8 + k) %/ 11] < 3329) => /= *. 
++ rewrite -Fq.Fq1024.compress_impl_large //=; 1: by rewrite /bpos16 qE /= /to_sint /smod /=;smt(W16.to_uint_cmp).  
+  congr;congr;congr;congr;congr;congr; 2: by smt().
+  rewrite /truncateu64_11 of_uintK /=. 
+  by rewrite /srl_64 /sll_64 /(`<<`) /(`>>`) /= /#.
+
+  
+have -> : (incoeff (to_sint p.[(8 * i + k) %/ 11])) = (incoeff (to_sint (W16_sub p.[(8 * i + k) %/ 11] (W16.of_int 3329)))); last first.
++ rewrite -Fq.Fq1024.compress_impl_large //=.
+  rewrite to_sintB_small /=;1: by rewrite  /(to_sint (W16.of_int 3329)) /= /smod /=;smt(size_map size_iota).
+  rewrite  /= /smod /= qE; have Hub := H00 ((8 * i + k) %/ 11) _; 1: by smt().
+  have E: to_sint (W16.of_int 3329) = 3329 by rewrite /to_sint /smod /=.
+  by rewrite E; smt(W16.to_uint_cmp pow2_16 W16.to_sintE qE).
+  rewrite /truncateu64_11 of_uintK /=.
+  by rewrite /srl_64 /sll_64 /(`<<`) /(`>>`) /= /#.
+
+rewrite -eq_incoeff.
+rewrite to_sintB_small /=;1: by rewrite  /(to_sint (W16.of_int 3329))/= /smod /=;smt(size_map size_iota). 
+   by rewrite  /(to_sint (W16.of_int 3329))  /= /smod /=; smt(size_map size_iota W16.to_uint_cmp).
+qed.
+
+lemma encode_vec_compress_bits (p : W16.t Array1024.t) (i : int) (k : int) :
+     0 <= i < 1024*11 %/ 8 =>
+     0 <= k < 8 =>
+    (ByteEncode 11 (to_list (compress_polyvec 11 (lift_polyvec p)))).[i].[k] =
+    ((Compress 11 (incoeff (to_sint p.[(8 * i + k) %/ 11])) %/ 2^((8 * i + k) %% 11)) %% 2 <> 0).
+move => Hi Hk.
+rewrite /ByteEncode /BitsToBytes (nth_map []).
++ rewrite size_chunk // (EclibExtra.size_flatten' 11);1: smt(mapP BS2Int.size_int2bs).
+  by rewrite size_map size_to_list /=; smt(kvec_val).
+rewrite /W8.bits2w initiE 1:/# /=.
+rewrite JWordList.nth_chunk 1,2:/#.
++ rewrite  (EclibExtra.size_flatten' 11);1: smt(mapP BS2Int.size_int2bs).
+  by rewrite size_map size_to_list /=; smt(kvec_val).
+rewrite nth_take 1,2:/# nth_drop 1,2:/#.
++ have -> := nth_flatten false 11; 1: by rewrite allP => ? /=;smt(mapP BS2Int.size_int2bs).
+rewrite (nth_map witness); 1: by rewrite size_to_list; smt(kvec_val).
+rewrite get_to_list /= /compress_polyvec (nth_map 0) /=;1:smt(size_iota).
+rewrite initiE; 1: by smt(kvec_val).
+rewrite /= nth_iota 1:/#.
+rewrite /lift_polyvec KVec.initiE; 1: by smt(kvec_val).
+simplify.
+rewrite /lift_array256 mapiE 1:/#.
+rewrite /= /subarray256 initiE 1:/#.
+simplify; have ->: 256 * ((8 * i + k) %/ 11 %/ 256) + (8 * i + k) %/ 11 %% 256 = (8 * i + k) %/ 11 by smt().
+done.
+qed.
+
+
+
+(********** BEGIN BDEP PROOF OF CSUBQ **************)
+
+abbrev keepodd11 = (W32.of_int 134152192).
+abbrev keepeven11 = (W32.of_int 2047).
+
+op VPMADDWD_alt(f0 m : W256.t) : W256.t =
+    if m <> (VPBROADCAST_4u64 (W64.of_int 576460756732608513)) then
+       VPMADDWD_256 f0 m
+    else
+    let f2 = VPBROADCAST_8u32 keepodd11 in
+    let f1 = VPAND_256 f0 f2  in
+    let f2 = VPBROADCAST_8u32 keepeven11 in
+    let f0 = VPAND_256 f0 f2  in
+    let f1 = VPSRL_8u32 f1  (W128.of_int 5) in
+        VPOR_256 f0 f1.
+
+
+lemma keepeven_bits b:
+  0 <= b < 32 =>
+   keepeven11.[b] <=> 0<=b<11.
+move => bb.
+have  : all (fun b => keepeven11.[b] <=> 0 <= b < 11) (iota_ 0 32); last by rewrite allP => H; move : (H b _); smt(mem_iota allP). 
+by rewrite /of_int  /int2bs /mkseq -iotaredE /=.
+qed.
+
+lemma keepodd_bits b: 
+  0 <= b < 32 =>
+   keepodd11.[b] <=> 16<=b<27.
+move => bb.
+have  : all (fun b => keepodd11.[b] <=> 16 <= b < 27) (iota_ 0 32); last by rewrite allP => H; move : (H b _); smt(mem_iota allP). 
+by rewrite /of_int  /int2bs /mkseq -iotaredE /=.
+qed.
+
+lemma lowbits_keep (f : W256.t) (i : int) (b : int) :
+  0 <= i < 16 => i %% 2 = 0 => 
+  0 <= b < 11 =>
+    (f \bits16 i).[b] = ((f \bits32 i%/2)  `&` keepeven11).[b].
+proof. 
+move => bi Hi Hb. 
+have H := W16u16.get_bits16 f (16*i + b) _;1:smt().
+have H0 := W8u32.get_bits32 f (16*i + b) _;1:smt().
+rewrite andE map2iE 1:/# /=.
+by smt(keepeven_bits).
+qed.
+
+lemma lowbits_drop (f : W256.t) (i : int) (b : int) :
+  0 <= i < 16 => i %% 2 = 0 => 
+  11 <= b < 16 =>
+  !((f \bits32 i%/2)  `&` keepeven11).[b].
+proof. 
+move => bi Hi Hb. 
+rewrite andE map2iE 1:/# /=.
+by smt(keepeven_bits).
+qed.
+
+lemma highbits_keep (f : W256.t) (i : int) (b : int) :
+  0 <= i < 16 => i %% 2 = 1 => 0 <= b < 11 =>
+    (f \bits16 i).[b] = ((f \bits32 i%/2)  `&` keepodd11).[b + 16].
+proof. 
+move => bi Hi Hb. 
+have H := W16u16.get_bits16 f (16*i + b) _;1:smt().
+have H0 := W8u32.get_bits32 f (16*i + b) _;1:smt().
+rewrite andE map2iE 1:/# /=.
+by smt(keepodd_bits).
+qed.
+
+lemma highbits_drop (f : W256.t) (i : int) (b : int) :
+  0 <= i < 16 => i %% 2 = 1 =>11 <= b < 15 =>
+    !((f \bits32 i%/2)  `&` keepodd11).[b + 16].
+proof. 
+move => bi Hi Hb. 
+rewrite andE map2iE 1:/# /=.
+by smt(keepodd_bits).
+qed.
+
+
+lemma lowbits_ofint_keep (f0 f1 : W16.t) b :
+  0 <= b < 11 =>
+  0<= to_sint f0 < 2048 =>
+  0<= to_sint f1 < 2048 =>
+  (W32.of_int (to_sint f0 + to_sint f1 * 2048)).[b] = f0.[b].
+move => ?.
+rewrite /to_sint /smod /= => ??.
+have  : all (fun b => (W32.of_int
+   ((if 32768 <= to_uint f0 then to_uint f0 - 65536 else to_uint f0) +
+    (if 32768 <= to_uint f1 then to_uint f1 - 65536 else to_uint f1) * 2048)).[b] =
+f0.[b]) (iota_ 0 11); last by rewrite allP => H; move : (H b _); smt(mem_iota allP). 
+ rewrite  /of_int /int2bs /mkseq -iotaredE /=;do split; rewrite get_to_uint /= /#.
+qed.
+
+lemma highbits_ofint_keep (f0 f1 : W16.t) b :
+  0<= to_sint f0 < 2048 =>
+  0<= to_sint f1 < 2048 =>
+  11 <= b < 22 =>
+  (W32.of_int (to_sint f0 + to_sint f1 * 2048)).[b] = f1.[b-11].
+move => ?.
+rewrite /to_sint /smod /= => ??.
+have  : all (fun b => (W32.of_int
+   ((if 32768 <= to_uint f0 then to_uint f0 - 65536 else to_uint f0) +
+    (if 32768 <= to_uint f1 then to_uint f1 - 65536 else to_uint f1) * 2048)).[b] =
+f1.[b - 11]) (iota_ 11 22); last by rewrite allP => H; move : (H b _); smt(mem_iota allP). 
+ rewrite  /of_int /int2bs /mkseq -iotaredE /=;do split; rewrite get_to_uint /=; smt(pow2_16 pow2_32). 
+qed.
+
+
+lemma highbits_ofint_drop (f0 f1 : W16.t) b :
+  0<= to_sint f0 < 2048 =>
+  0<= to_sint f1 < 2048 =>
+  22 <= b < 32 =>
+  !(W32.of_int (to_sint f0 + to_sint f1 * 2048)).[b].
+move => ?.
+rewrite /to_sint /smod /= => ??.
+have  : all (fun b => ! (W32.of_int
+     ((if 32768 <= to_uint f0 then to_uint f0 - 65536 else to_uint f0) +
+      (if 32768 <= to_uint f1 then to_uint f1 - 65536 else to_uint f1) * 2048)).[b]) (iota_ 22 32); last by rewrite allP => H; move : (H b _); smt(mem_iota allP). 
+ rewrite  /of_int /int2bs /mkseq -iotaredE /=;do split; smt(pow2_16 pow2_32). 
+qed.
+
+
+lemma unand (f : W256.t) (i : int) (b : int) :
+  0 <= i < 8 => 0<=b<32 =>
+   (W32.init (fun (j : int) => (f \bits32 i).[j + 5] /\ keepodd11.[j + 5])).[b] = ((f \bits32 i) `&` keepodd11).[b + 5].
+proof.
+move => ??.
+by rewrite initiE 1:/# /=.
+qed.
+
+lemma vpmaddwd_alt_corr (f0 shift2 : W256.t) :
+   (forall i, 0 <= i < 16 => 0<= to_sint (f0 \bits16 i) < 2^11) =>
+   VPMADDWD_256 f0 shift2 = VPMADDWD_alt f0 shift2.
++ move => /= H;rewrite /VPMADDWD_256 /VPMADDWD_alt /=. 
+  case (shift2 = VPBROADCAST_4u64 pvc_shift2_s);2: by auto. 
+  move => -> /=; rewrite /VPBROADCAST_4u64 /= -!(iotaredE) /=. 
+  pose f00 := (f0 \bits16 0).
+  pose f01 := (f0 \bits16 1).
+  pose f02 := (f0 \bits16 2).
+  pose f03 := (f0 \bits16 3).
+  pose f04 := (f0 \bits16 4).
+  pose f05 := (f0 \bits16 5).
+  pose f06 := (f0 \bits16 6).
+  pose f07 := (f0 \bits16 7).
+  pose f08 := (f0 \bits16 8).
+  pose f09 := (f0 \bits16 9).
+  pose f010 := (f0 \bits16 10).
+  pose f011 := (f0 \bits16 11).
+  pose f012 := (f0 \bits16 12).
+  pose f013 := (f0 \bits16 13).
+  pose f014 := (f0 \bits16 14).
+  pose f015 := (f0 \bits16 15).
+  rewrite  /(\bits16) /= !W16.init_bits2w -!iotaredE /= /W64.of_int /= /int2bs /mkseq -!iotaredE /=; do 16!(rewrite /(to_sint (W16.bits2w _)) /smod /= /(W16.to_uint (W16.bits2w (_::_)))). 
+  rewrite  !bits2wK //= !JUtils.bs2int_cons /b2i /= !bs2int_nil /=.
+  rewrite !hadd_cons2 hadd_nil /=.
+  rewrite /VPBROADCAST_8u32 -!iotaredE /= /VPSRL_8u32 /= /(`>>>`) /= -(unpack32K f0) andb8u32E !orb8u32E;congr;rewrite /unpack32 init_of_list -iotaredE /= orE.
+  congr;apply (eq_from_nth witness) => //= => i ib. 
+  apply W32.wordP => b bb. 
+  have /= H3 := highbits_keep f0 (i*2+1) (b-11) _ _;1,2: smt().
+  have /= H4 := highbits_drop f0 (i*2+1) (b-11) _ _;1,2: smt().
+  have /= H5 := lowbits_keep f0  (i*2) b _ _;1,2: smt().
+  have /= H6 := lowbits_drop f0 (i*2) b _ _;1,2: smt(). 
+  case (i = 0) => *.
+  + rewrite map2iE 1:/# unand 1,2:/#.
+    have /= H0 := highbits_ofint_drop f00 f01 b _ _;1,2:smt().
+    have /= H1 := highbits_ofint_keep f00 f01 b _ _;1,2:smt().
+    have /= H2 := lowbits_ofint_keep f00 f01 b.
+    smt(keepodd_bits keepeven_bits W32.get_out).
+  case (i - 1 = 0) => *.
+  + rewrite map2iE 1:/# unand 1,2:/#.
+    have /= H0 := highbits_ofint_drop f02 f03 b _ _;1,2:smt().
+    have /= H1 := highbits_ofint_keep f02 f03 b _ _;1,2:smt().
+    have /= H2 := lowbits_ofint_keep f02 f03 b.
+    smt(keepodd_bits keepeven_bits W32.get_out).
+  case (i - 2 = 0) => *.
+  + rewrite map2iE 1:/# unand 1,2:/#.
+    have /= H0 := highbits_ofint_drop f04 f05 b _ _;1,2:smt().
+    have /= H1 := highbits_ofint_keep f04 f05 b _ _;1,2:smt().
+    have /= H2 := lowbits_ofint_keep f04 f05 b.
+    smt(keepodd_bits keepeven_bits W32.get_out).
+  case (i - 3 = 0) => *.
+  + rewrite map2iE 1:/# unand 1,2:/#.
+    have /= H0 := highbits_ofint_drop f06 f07 b _ _;1,2:smt().
+    have /= H1 := highbits_ofint_keep f06 f07 b _ _;1,2:smt().
+    have /= H2 := lowbits_ofint_keep f06 f07 b.
+    smt(keepodd_bits keepeven_bits W32.get_out).
+  case (i - 4 = 0) => *.
+  + rewrite map2iE 1:/# unand 1,2:/#.
+    have /= H0 := highbits_ofint_drop f08 f09 b _ _;1,2:smt().
+    have /= H1 := highbits_ofint_keep f08 f09 b _ _;1,2:smt().
+    have /= H2 := lowbits_ofint_keep f08 f09 b.
+    smt(keepodd_bits keepeven_bits W32.get_out).
+  case (i - 5 = 0) => *.
+  + rewrite map2iE 1:/# unand 1,2:/#.
+    have /= H0 := highbits_ofint_drop f010 f011 b _ _;1,2:smt().
+    have /= H1 := highbits_ofint_keep f010 f011 b _ _;1,2:smt().
+    have /= H2 := lowbits_ofint_keep f010 f011 b.
+    smt(keepodd_bits keepeven_bits W32.get_out).
+  case (i - 6 = 0) => *.
+  + rewrite map2iE 1:/# unand 1,2:/#.
+    have /= H0 := highbits_ofint_drop f012 f013 b _ _;1,2:smt().
+    have /= H1 := highbits_ofint_keep f012 f013 b _ _;1,2:smt().
+    have /= H2 := lowbits_ofint_keep f012 f013 b.
+    smt(keepodd_bits keepeven_bits W32.get_out).
+  case (i - 7 = 0) => *.
+  + rewrite map2iE 1:/# unand 1,2:/#.
+    have /= H0 := highbits_ofint_drop f014 f015 b _ _;1,2:smt().
+    have /= H1 := highbits_ofint_keep f014 f015 b _ _;1,2:smt().
+    have /= H2 := lowbits_ofint_keep f014 f015 b.
+    smt(keepodd_bits keepeven_bits W32.get_out).
+by smt().
+qed.
+
