proof/correctness/avx2/768/MLKEM_PolyVec_avx2_circuit.ec
@@ -1,0 +1,768 @@
+require import AllCore List Int IntDiv CoreMap Real Number Ring StdOrder BitEncoding.
+
+from Jasmin require import JModel.
+from JazzEC require import Array2304 Array1536 Array1408 Array1152 Array1088 Array1024 Array960 Array768 Array400 Array384 Array256 Array160 Array128 Array64 Array32 Array16 Array8 Array4 Array2.
+from JazzEC require import WArray1536 WArray1410 WArray1152 WArray960 WArray512 WArray384 WArray160 WArray128 WArray32 WArray16.
+from JazzEC require import Jkem_avx2.
+
+require import AVX2_Ops W16extra.
+require import Fq NTT_Fq MLKEMFCLib MLKEM_W16_Rep MLKEM768_prelude.
+require import Fq_avx2 NTT_avx2 NTT_avx2_poly AVX2_Ops MLKEMFCLib.
+require import MLKEM_Poly_avx2 MLKEM_PolyVec_avx2.
+require import MLKEM_Poly_avx2_circuit MLKEM_Poly_avx2_circuit_768.
+require import Mlkem_bindings.
+require import Circuit_semantics Circuit_sem_768.
+from Spec require import GFq Rq Serialization VecMat Sampling EncDecCorrectness Correctness.
+
+import BitChunking BS2Int.
+import Fq.
+import GFq Rq Serialization VecMat.
+import Zq ZModP.
+import Fq_avx2 NTT_Avx2.
+import MLKEMFCLib768.
+import MLKEM_PolyAVX MLKEM_PolyvecAVX MLKEM_PolyAVXVec.
+import PolyVec PolyMat.
+import W12.
+
+abbrev encode10_vec (a : ipolyvec) : W8.t Array960.t = Array960.of_list W8.zero (ByteEncode 10 (to_list a)).
+
+
+lemma polyvec_csubq_avx2_ll :
+   islossless Jkem_avx2.M.__polyvec_csubq.
+by proc;inline *;do 4!(unroll for ^while);auto.
+qed.
+
+lemma polyvec_csubq_avx2_corr_h (_aw : W16.t Array768.t):
+    hoare[ Jkem_avx2.M.__polyvec_csubq  :
+             r = _aw /\
+             pos_bound768_cxq r 0 768 2 ==> 
+             lift_array768 res = lift_array768 _aw /\
+             pos_bound768_cxq res 0 768 1]. 
+proof.
+proc; inline *.
+proc change ^while.1: {rp <- init_256_16 (fun i0 => r.[256*i+i0]);};1: by auto.
+proc change ^while.2: {qx16 <- sliceget16_16_256 jqx16 0;}; 1: by auto.
+proc change ^while.^while.1: {r0 <- sliceget256_16_256 rp (i0*256);};1: by auto => /#.
+proc change ^while.^while.9: {rp <- sliceset256_16_256 rp (i0*256) r0;};1: by auto => /#.
+proc change ^while.6: {r <- init_768_16 (fun (i_0 : int) => if 256 * i <= i_0 < 256 * i + 256 then aux.[i_0 - 256 * i] else r.[i_0]);};1: by auto. 
+
+do 4!(unroll for ^while).
+cfold ^i0<-.
+wp -2.
+
+conseq (: r = _aw /\ all (fun c => W16.zero \sle c && c \slt W16.of_int 6658) r ==>
+       r = init_768_16 (fun i => csubq_circuit _aw.[i])); last by circuit.
+
+       
+(* BDEP pre conseq *)
++ move => &hr />. rewrite /pos_bound768_cxq /bpos16 qE /= => H.
+  rewrite /(\slt) /(\sle) /= /smod /= allP /=.
+  by exact H.
+
+(* BDEP post conseq *)
+
+(* We start with some boilerplate *)
+move => &hr [#]/= ->; rewrite /pos_bound256_cxq => Hb rr; rewrite /init_768_16 /lift_array768 /= => ->; split.
+
+rewrite tP => i ib.
+rewrite !mapiE 1,2:/# /= initiE 1:/# /=.
+rewrite /csubq_circuit ultE /W16_sub /=.
+move : (Hb i ib);rewrite /bpos16 qE /= /to_sint /smod /=.
+case (to_uint _aw.[i] < 3329) => *//;1:
+have ->/= : !32768 <= to_uint _aw.[i] by smt(W16.to_uint_cmp).
+rewrite to_uintB /=;1: by rewrite uleE => /#.
+have ->/= : !32768 <= to_uint _aw.[i] - 3329;  by smt(W16.to_uint_cmp).
+
+move => i ib.
+rewrite initiE 1:/# /= /csubq_circuit ultE /W16_sub /=.
+move : (Hb i ib);rewrite /bpos16 qE /= /to_sint /smod /=.
+case (to_uint _aw.[i] < 3329) => *//;1:
+have ->/= : !32768 <= to_uint _aw.[i] by smt(W16.to_uint_cmp).
+by smt(W16.to_uint_cmp).
+rewrite to_uintB /=;1: by rewrite uleE => /#.
+have ->/= : !32768 <= to_uint _aw.[i] - 3329;  by smt(W16.to_uint_cmp).
+qed.
+
+lemma polyvec_csubq_avx2_corr (_aw : W16.t Array768.t):
+    phoare[ Jkem_avx2.M.__polyvec_csubq  :
+             r = _aw /\
+             pos_bound768_cxq r 0 768 2 ==> 
+             lift_array768 res = lift_array768 _aw /\
+             pos_bound768_cxq res 0 768 1] = 1%r
+  by conseq polyvec_csubq_avx2_ll (polyvec_csubq_avx2_corr_h _aw).
+
+
+
+(********** END BDEP PROOF OF CSUBQ **************)
+
+
+lemma polyvec_decompress_ll :
+   islossless Jkem_avx2.M.__i_polyvec_decompress.
+by proc;inline *;unroll for ^while; do 3!(cfold ^inc<-; unroll for ^while);auto.
+qed.
+(********** BEGIN BDEP PROOF OF DECOMPRESS **************)
+
+lemma polyvec_decompress_corr_h (_aw : W8.t Array960.t):
+    hoare[ Jkem_avx2.M.__i_polyvec_decompress :
+             Array960.init (fun i => rp.[i]) = _aw ==> pos_bound768_cxq res 0 768 1 /\ lift_polyvec res = decompress_polyvec 10 (decode10_vec _aw)].
+proc; inline *.
+proc change 3: { shufbidx <- sliceget32_8_256 pvd_shufbdidx_s 0;}; 1: by auto.
+proc change ^while.^while.1 : {f <- sliceget1088_8_256 rp ((320*k + 20*i)*8);}; 1: by auto => /> /#.
+proc change ^while.^while.8 : {r <- sliceset768_16_256 r ((16 * k + i)*256) f;}; 1: by auto => /> /#.
+unroll for ^while.
+cfold ^inc<-.
+do 3!(unroll for ^while).
+cfold ^i<-.
+wp -3.
+
+
+conseq (: rp = init_1088_8 (fun i => if i < 960 then _aw.[i] else rp.[i])
+        ==>
+   r = init_768_16 (fun i =>
+     decompress10_circuit (W10.init (fun (j : int) => _aw.[(i*10 + j) %/ 8].[(i*10 + j) %% 8]))));last  circuit. 
+     
+(* We start with some boilerplate *)
+move => &hr /=;rewrite !tP  => H i ib.
+by rewrite initE ib /=; case (i < 960) => // ?; rewrite -H 1:/# initiE 1:/#.
+
+move => &hr <- rr ->; split; last first.
++ rewrite KVec.tP => k kb.
+  rewrite tP => i ib.
+  rewrite /lift_polyvec /init_768_16 KVec.initiE 1:/# /= !mapiE 1:/# /= -get_to_list /= initiE 1:/# /= initiE 1:/# /=.
+  rewrite initiE; 1: by smt(kvec_val).
+  simplify.
+  rewrite mapiE 1:/#.
+  rewrite /subarray256 initiE 1:/#.
+  simplify.
+  rewrite decompress10_circuit_sem; 1: by smt(kvec_val).
+  done.
+
+  
+rewrite /pos_bound768_cxq qE /= => k kb. 
+rewrite /init_768_16 initiE 1:/# /=.
+by apply decompress10_circuit_rng.
+qed.
+
+
+
+lemma polyvec_decompress_corr (_aw : W8.t Array960.t):
+    phoare[ Jkem_avx2.M.__i_polyvec_decompress :
+             Array960.init (fun i => rp.[i]) = _aw ==> pos_bound768_cxq res 0 768 1 /\ lift_polyvec res = decompress_polyvec 10 (decode10_vec _aw)] = 1%r
+ by conseq polyvec_decompress_ll (polyvec_decompress_corr_h _aw).
+
+(********** BEGIN BDEP PROOF OF COMPRESS  **************)
+
+module AuxCompress10 = {
+
+proc __i_polyvec_compress(rp : W8.t Array960.t, a : W16.t Array768.t) : W8.t Array960.t = {
+    var inc : int;
+    var x16p : W16.t Array16.t;
+    var v : W256.t;
+    var v8 : W256.t;
+    var off : W256.t;
+    var shift1 : W256.t;
+    var mask : W256.t;
+    var shift2 : W256.t;
+    var sllvdidx : W256.t;
+    var shufbidx : W256.t;
+    var i : int;
+    var f0 : W256.t;
+    var f1 : W256.t;
+    var f2 : W256.t;
+    var t0 : W128.t;
+    var t1 : W128.t;
+    x16p <- witness;
+    a <@ M.__polyvec_csubq(a);
+    x16p <- jvx16;
+    v <- get256 (WArray32.init16 (fun (i_0 : int) => x16p.[i_0])) 0;
+    v8 <- VPSLL_16u16 v (W128.of_int 3);
+    off <- VPBROADCAST_16u16 pc_mask_s;
+    shift1 <- VPBROADCAST_16u16 pvc_shift1_s;
+    mask <- VPBROADCAST_16u16 pvc_mask_s;
+    shift2 <- VPBROADCAST_4u64 pvc_shift2_s;
+    sllvdidx <- VPBROADCAST_4u64 pvc_sllvdidx_s;
+    shufbidx <- get256 (WArray32.init8 (fun (i_0 : int) => pvc_shufbidx_s.[i_0])) 0;
+    inc <- 3 * 256 %/ 16;
+    i <- 0;
+    while (i < inc){
+      f0 <- get256 (WArray1536.init16 (fun (i_0 : int) => a.[i_0])) i;
+      f1 <- VPMULL_16u16 f0 v8;
+      f2 <- VPADD_16u16 f0 off;
+      f0 <- VPSLL_16u16 f0 (W128.of_int 3);
+      f0 <- VPMULH_16u16 f0 v;
+      f2 <- VPSUB_16u16 f1 f2;
+      f1 <- invw f1 `&` f2;
+      f1 <- VPSRL_16u16 f1 (W128.of_int 15);
+      f0 <- VPSUB_16u16 f0 f1;
+      f0 <- VPMULHRS_16u16 f0 shift1;
+      f0 <- f0 `&` mask;
+      f0 <- VPMADDWD_alt f0 shift2;
+      f0 <- VPSLLV_8u32 f0 sllvdidx;
+      f0 <- VPSRL_4u64 f0 (W128.of_int 12);
+      f0 <- VPSHUFB_256 f0 shufbidx;
+      t0 <- truncateu128 f0;
+      t1 <- VEXTRACTI128 f0 W8.one;
+      t0 <- VPBLENDW_128 t0 t1 (W8.of_int 224);
+      rp <-
+        Array960.init
+          (WArray960.get8
+             (WArray960.set128_direct (WArray960.init8 (fun (i_0 : int) => rp.[i_0])) (20 * i) t0));
+      rp <-
+        Array960.init
+          (WArray960.get8
+             (WArray960.set32_direct (WArray960.init8 (fun (i_0 : int) => rp.[i_0])) (
+                20 * i + 16) (VPEXTR_32 t1 W8.zero)));
+      i <- i + 1;
+    }
+    
+    return rp;
+  }
+}.
+
+lemma auxcompress10_ll : islossless AuxCompress10.__i_polyvec_compress.
+proc. cfold 12. unroll for ^while; wp => /=. 
+inline *;unroll for ^while; do 3!(unroll for ^while);auto.
+qed.
+
+lemma auxcompress10_corr_h (_aw : W16.t Array768.t):
+    hoare[ AuxCompress10.__i_polyvec_compress  :
+             a = _aw /\
+             pos_bound768_cxq a 0 768 2 ==> 
+      res = encode10_vec (compress_polyvec 10 (lift_polyvec _aw))].
+proof.
+proc; inline *.
+proc change ^while.1: { rp0 <- init_256_16 (fun i => r.[256*i0+i]);};1: by auto.
+proc change ^while.2: { qx16 <- sliceget16_16_256 jqx16 0;}; 1: by auto.
+proc change ^while.^while.1: {r0 <- sliceget256_16_256 rp0 (i1*256);};1: by auto => /#.
+proc change ^while.^while.9: { rp0 <- sliceset256_16_256 rp0 (i1*256) r0;};1: by auto => /#.
+proc change ^while.6: { r <- init_768_16 (fun (i_0 : int) => if 256 * i0 <= i_0 < 256 * i0 + 256 then aux.[i_0 - 256 * i0] else r.[i_0]);};1: by auto. 
+proc change 7: { v <- sliceget16_16_256 x16p 0;}; 1: by auto.
+proc change ^while{2}.1: {f0 <- sliceget768_16_256 a (i*256);};1: by auto => /#.
+proc change 14: { shufbidx <- sliceget32_8_256 pvc_shufbidx_s 0;}; 1: by auto.
+proc change ^while{2}.19 : { rp <- sliceset960_8_128 rp  (20*i*8) t0;};1: by auto => /#.
+proc change ^while{2}.20 : { rp <- sliceset960_8_32 rp  ((20*i+16)*8) (truncateu32 t1);}.
++ auto => />;move => *;rewrite /sliceset960_8_32 tP => *.
+  rewrite initiE /= 1:/# ifT 1:/# initiE 1:/#.
+  do congr;1: smt(). 
+  by rewrite /VPEXTR_32 /truncateu32 to_uint_eq /= bits32_div //.
+unroll for ^while.
+do 3!(unroll for ^while).
+cfold ^inc<-.
+unroll for ^while.
+cfold ^i0<-. 
+cfold ^i1<-. 
+wp -4.
+
+conseq (: a = _aw /\
+   Array768.all (fun bv => W16.zero \sle bv /\ bv \slt (of_int (2 * 3329))) a
+   ==> rp = init_960_8 (fun i =>
+     W8.init (fun j =>
+       (compress10_circuit _aw.[(i*8+j) %/ 10]).[(i*8+j) %% 10]))); last by circuit.
+
+      
+(* BDEP pre conseq *)
++ move => &hr />; rewrite /pos_bound768_cxq qE /= /(\sle) /(\slt) allP /=  => Hb i ib /=.
+  rewrite /(to_sint W16.zero) /= /(W16.smod 0) /=.
+  rewrite /(to_sint (W16.of_int 6658)) /= /(W16.smod 6658) /= /#.
+  
+(* BDEP post conseq *)
+
+(* We start with some boilerplate *)
+move => &hr [#]/= -> H0 rr; rewrite /= /init_960_8 !tP => H i ib.
+rewrite H // initiE 1:/# /=.
+rewrite wordP => k kb; rewrite !initiE /= 1,2:/#.
+rewrite encode_vec_compress_bits //=.
+by apply compress10_circuit_sem.
+qed.
+
+(********** END BDEP PROOF OF COMPRESS **************)
+
+lemma auxcompress10_corr (_aw : W16.t Array768.t):
+    phoare[ AuxCompress10.__i_polyvec_compress  :
+             a = _aw /\
+             pos_bound768_cxq a 0 768 2 ==> 
+      res  = encode10_vec (compress_polyvec 10 (lift_polyvec _aw))] = 1%r 
+  by conseq auxcompress10_ll (auxcompress10_corr_h _aw).
+
+
+lemma polyvec_compress_avx2_ll : islossless Jkem_avx2.M.__i_polyvec_compress.
+proc. cfold 12. unroll for ^while; wp => /=. 
+inline *;unroll for ^while; do 3!(unroll for ^while);auto.
+qed.
+
+lemma polyvec_compress_avx2_corr (_aw : W16.t Array768.t):
+    phoare[ Jkem_avx2.M.__i_polyvec_compress  :
+             a = _aw /\
+             pos_bound768_cxq a 0 768 2 ==> 
+      res  = encode10_vec (compress_polyvec 10 (lift_polyvec _aw))] = 1%r.
+bypr => &m [->?].
+have <- : Pr[ AuxCompress10.__i_polyvec_compress(rp{m}, _aw) @ &m :
+   res = encode10_vec (compress_polyvec 10 (lift_polyvec _aw))] = 1%r
+   by byphoare (auxcompress10_corr _aw)  =>/=;1:smt().
+byequiv (: ={arg} /\ a{1} = _aw /\
+             pos_bound768_cxq a{1} 0 768 2 ==> ={res}) => //.
+proc.
+seq 2 2 : (={rp,a} /\ pos_bound768_cxq a{1} 0 768 1).
++ ecall {1} (polyvec_csubq_avx2_corr a{1}). 
+  ecall {2} (polyvec_csubq_avx2_corr a{2}). 
+  auto => />; rewrite /pos_bound768_cxq /lift_array768 /= qE /= => ? rr1.
+  rewrite !tP;move =>  Hrr11 Hrr12 rr2.
+  rewrite !tP;move =>  Hrr21 Hrr22.
+  move => i ib. 
+  have := Hrr11 i ib; rewrite !mapiE 1,2:/# /=. 
+  have := Hrr12 i ib.  
+  have := Hrr21 i ib; rewrite !mapiE 1,2:/# /=. 
+  have := Hrr22 i ib.  
+  rewrite /to_sint /smod /=. 
+  move => Hrr11i Hrr12i Hrr21i Hrr22i.
+  have Hn1 : !(32768 <= to_uint rr2.[i]) by smt(W16.to_uint_cmp pow2_16).
+  have Hn2 : !(32768 <= to_uint rr1.[i]) by smt(W16.to_uint_cmp pow2_16).
+  have Hn3 : !(32768 <= to_uint _aw.[i]) by smt(W16.to_uint_cmp pow2_16).
+  move : Hrr11i Hrr12i Hrr21i Hrr22i; rewrite Hn1 Hn2 Hn3 /=.
+  move => Hrr11i Hrr12i Hrr21i Hrr22i.
+  move : Hrr12i; rewrite -Hrr22i -eq_incoeff.  
+  by rewrite !modz_small ?qE /= 1,2:/# to_uint_eq /#.
+
+cfold {1} ^inc<-. 
+cfold {2} ^inc<-. 
+sp 9 9.
+wp;while (#pre /\ ={i} /\ 0 <= i{1} <=64); last by auto.
+wp -1 -1; conseq (: _ ==> ={rp}); 1: by auto => /#.
+sim;conseq />.
+seq 10 10 : (#pre /\ ={f0}); 1: by conseq />;sim.
+auto => /> &1;rewrite vpmaddwd_alt_corr; last by rewrite /VPMADDWD_alt /=.
+move => i ib /=; rewrite /VPBROADCAST_16u16 /=.
+rewrite Montgomery16.bits16_W16u16 ib /= get_of_list 1:/# /= (nth_map witness) /=;1:smt(size_iota).
+have -> : 1023 = 2^10 -1 by auto.
+rewrite and_mod 1:/# /= /smod /= /#.
+qed.
+
+lemma polyvec_frombytes_ll : islossless Jkem_avx2.M.__i_polyvec_frombytes.
+proc; inline *;wp. 
+  while (0 <= i <= 4) (4-i); last by  auto =>  /> /#.
+move => *. cfold 3. unroll for ^while;auto => /> /#.
+qed.
+
+op nttunpack_16 (rp : W16.t Array256.t) : W16.t Array256.t = init_256_16 (fun (i : int) => rp.[nttunpack_idx.[i]]).
+
+
+op nttunpackv_16 (v : W16.t Array768.t) : W16.t Array768.t =
+  init_768_16
+    (fun (i : int) =>
+       if 0 <= i < 256 then (nttunpack_16 (subarray256 v 0)).[i]
+       else
+         if 256 <= i < 512 then (nttunpack_16 (subarray256 v 1)).[i - 256]
+         else  (nttunpack_16 (subarray256 v 2)).[i - 512]).
+
+lemma nttunpackv_16E v: nttunpackv_16 v = nttunpackv v.
+   rewrite /nttunpackv_16 /nttunpackv /nttunpack_16 /nttunpack.
+   by rewrite /init_768_16 /init_256_16.
+   qed.
+
+
+lemma polyvec_frombytes_corr_h (_aw : W8.t Array1152.t): 
+    hoare [Jkem_avx2.M.__i_polyvec_frombytes  :
+             a = _aw
+              ==>
+             lift_array768 res = nttunpackv (map incoeff (Array768.of_list 0 (ByteDecode 12 (to_list _aw))))  /\
+             pos_bound768_cxq res 0 768  2].
+proc; inline *.
+proc change ^while.1: { rp <- init_256_16 (fun (i_0 : int) => r.[256 * i + i_0]);}; 1: by auto.
+proc change ^while.2: { ap <- init_384_8 (fun (i_0 : int) => a.[384 * i + i_0]);}; 1: by auto.
+proc change ^while.3: { mask <- sliceget16_16_256 maskx16 0;}; 1: by auto.
+proc change ^while.^while.1 : { t0 <- sliceget384_8_256 ap (192*i0*8);}; 1: by auto => /> /#.
+proc change ^while.^while.2 : { t1 <- sliceget384_8_256 ap ((192*i0+32)*8);}; 1: by auto => /> /#.
+proc change ^while.^while.3 : { t2 <- sliceget384_8_256 ap ((192*i0+64)*8);}; 1: by auto => /> /#.
+proc change ^while.^while.4 : { t3 <- sliceget384_8_256 ap ((192*i0+96)*8);}; 1: by auto => /> /#.
+proc change ^while.^while.5 : { t4 <- sliceget384_8_256 ap ((192*i0+128)*8);}; 1: by auto => /> /#.
+proc change ^while.^while.6 : { t5 <- sliceget384_8_256 ap ((192*i0+160)*8);}; 1: by auto => /> /#.
+proc change ^while.^while.101 : { rp <- sliceset256_16_256 rp (8*i0 *256) t6;};1: by auto => /> /#.
+proc change ^while.^while.102 : { rp <- sliceset256_16_256 rp ((8*i0+1) *256) t7;};1: by auto => /> /#.
+proc change ^while.^while.103 : { rp <- sliceset256_16_256 rp ((8*i0+2) *256) t8;};1: by auto => /> /#.
+proc change ^while.^while.104 : { rp <- sliceset256_16_256 rp ((8*i0+3) *256) t9;};1: by auto => /> /#.
+proc change ^while.^while.105 : { rp <- sliceset256_16_256 rp ((8*i0+4) *256) t4;};1: by auto => /> /#.
+proc change ^while.^while.106 : { rp <- sliceset256_16_256 rp ((8*i0+5) *256) t10;};1: by auto => /> /#.
+proc change ^while.^while.107 : { rp <- sliceset256_16_256 rp ((8*i0+6) *256) t11;};1: by auto => /> /#.
+proc change ^while.^while.108 : { rp <- sliceset256_16_256 rp ((8*i0+7) *256) tt;};1: by auto => /> /#.
+proc change ^while.7: { r <- init_768_16 (fun (i_0 : int) => if 256 * i <= i_0 < 256 * i + 256 then aux.[i_0 - 256 * i] else r.[i_0]);}; 1: by auto.
+
+unroll for ^while.
+do 3!(unroll for ^while).
+cfold ^i0<-.
+wp -2. 
+
+conseq (: _ ==> r = nttunpackv_16 (init_768_16 (fun i =>
+     frombytes_circuit (
+       W12.init (fun j =>
+         let idx = i*12 + j in
+         let aidx = idx %/ 8 in
+         let bidx = idx %% 8 in
+         _aw.[aidx].[bidx]
+       )
+     )))); last by  circuit.
+     
+move => &hr <- rr ->.
+rewrite nttunpackv_16E;split.
++ rewrite  -nttunpackv_lift /lift_array768 /=; congr; apply Array768.tP => i ib.
+  rewrite mapiE 1:/# /init_768_16 initiE 1:/#.
+  simplify.
+  rewrite frombytes_circuit_sem; 1: by smt().
+  rewrite get_of_list; 1: by smt(kvec_val).
+  rewrite get_of_list 1:/#.
+  rewrite (nth_map 0).
+  by rewrite /ByteDecode size_map size_chunk // size_BytesToBits size_to_list /#.
+  done.
+
+rewrite /pos_bound768_cxq.
+move => k kb.
+have : Array768.all (fun w => bpos16 w (2*q))
+    (nttunpackv
+       (init_768_16
+          (fun (i : int) =>
+             frombytes_circuit
+               (W12.init
+                  (fun (j : int) =>
+                     let idx = i * 12 + j in let aidx = idx %/ 8 in let bidx = idx %% 8 in a{hr}.[aidx].[bidx]))))); last first.
+ + by rewrite allP => H; have /= := H k _;1:smt().
+ 
+   
+apply nttunpackv_pred.
+rewrite allP => i ib; rewrite initiE 1:/# /= qE /=.
+have := frombytes_circuit_rng a{hr} i.
+smt().
+qed.
+
+
+(********** END BDEP PROOF OF FROMBYTES **************)
+
+lemma polyvec_frombytes_corr (_aw : W8.t Array1152.t): 
+    phoare [Jkem_avx2.M.__i_polyvec_frombytes  :
+             a = _aw
+              ==>
+             lift_array768 res = nttunpackv (map incoeff (Array768.of_list 0 (ByteDecode 12 (to_list _aw))))  /\
+             pos_bound768_cxq res 0 768  2] = 1%r
+  by conseq polyvec_frombytes_ll (polyvec_frombytes_corr_h _aw).
+
+op pcond_reduced (w: W16.t) =   w \ult W16.of_int (2*3329).
+
+lemma polyvec_tobytes_ll : islossless Jkem_avx2.M.__i_polyvec_tobytes.
+proc.
+inline *. 
+do 7!(unroll for ^while); auto. 
+qed.
+
+abbrev mask12 = VPBROADCAST_16u16(W16.of_int 4095).
+
+module AuxToBytes = {
+proc __i_polyvec_tobytes(r : W8.t Array1152.t, a : W16.t Array768.t) : W8.t Array1152.t = {
+  var i,rp,a0,i0,t0,t1,t2,t3,t4,t5,t6,t7,tt,ttt,a1,b,t00,r00,t10,r1,a2,b0,t01,r01,t11,r10,a3,b1,t02,r02,t12,r11,a4,b2,t03,t13,a5,b3,t04,t14,a6,b4,t05,t15,a7,b5,r03,r12,a8,b6,r04,r13,a9,b7,r05,r14,a10,b8,r06,r15,a11,b9,r07,r16,a12,b10,r08,r17,aux,aux_0;
+  i <- 0;                                                                                                                       
+  while (i < 3) {                                                                                                              
+    rp <- Array384.init (fun (i_0 : int) => r.[384 * i + i_0]);                                                                 
+    a0 <- Array256.init (fun (i_0 : int) => a.[256 * i + i_0]);  
+    a0 <@ Jkem_avx2.M._poly_csubq(a0);                                                           
+    i0 <- 0;                                                                                                                    
+    while (i0 < 2) {                                                                                                           
+      t0 <- get256 (WArray512.init16 (fun (i_0 : int) => a0.[i_0])) (8 * i0);                                                   
+      t1 <- get256 (WArray512.init16 (fun (i_0 : int) => a0.[i_0])) (8 * i0 + 1);                                               
+      t2 <- get256 (WArray512.init16 (fun (i_0 : int) => a0.[i_0])) (8 * i0 + 2);                                               
+      t3 <- get256 (WArray512.init16 (fun (i_0 : int) => a0.[i_0])) (8 * i0 + 3);                                               
+      t4 <- get256 (WArray512.init16 (fun (i_0 : int) => a0.[i_0])) (8 * i0 + 4);                                               
+      t5 <- get256 (WArray512.init16 (fun (i_0 : int) => a0.[i_0])) (8 * i0 + 5);                                               
+      t6 <- get256 (WArray512.init16 (fun (i_0 : int) => a0.[i_0])) (8 * i0 + 6);                                               
+      t7 <- get256 (WArray512.init16 (fun (i_0 : int) => a0.[i_0])) (8 * i0 + 7);                                               
+      t0 <- t0 `&` mask12;                                                                                                      
+      t1 <- t1 `&` mask12;                                                                                                      
+      t2 <- t2 `&` mask12;                                                                                                      
+      t3 <- t3 `&` mask12;                                                                                                      
+      t4 <- t4 `&` mask12;                                                                                                      
+      t5 <- t5 `&` mask12;                                                                                                      
+      t6 <- t6 `&` mask12;                                                                                                      
+      t7 <- t7 `&` mask12;                                                                                                      
+      tt <- VPSLL_16u16 t1 (W128.of_int 12);                                                                                    
+      tt <- tt `|` t0;                                                                                                          
+      t0 <- VPSRL_16u16 t1 (W128.of_int 4);                                                                                     
+      t1 <- VPSLL_16u16 t2 (W128.of_int 8);                                                                                     
+      t0 <- t0 `|` t1;                                                                                                          
+      t1 <- VPSRL_16u16 t2 (W128.of_int 8);                                                                                     
+      t2 <- VPSLL_16u16 t3 (W128.of_int 4);                                                                                     
+      t1 <- t1 `|` t2;                                                                                                          
+      t2 <- VPSLL_16u16 t5 (W128.of_int 12);                                                                                    
+      t2 <- t2 `|` t4;                                                                                                          
+      t3 <- VPSRL_16u16 t5 (W128.of_int 4);                                                                                     
+      t4 <- VPSLL_16u16 t6 (W128.of_int 8);                                                                                     
+      t3 <- t3 `|` t4;                                                                                                         
+      t4 <- VPSRL_16u16 t6 (W128.of_int 8);                                                                                     
+      t5 <- VPSLL_16u16 t7 (W128.of_int 4);                                                                                     
+      t4 <- t4 `|` t5;                                                                                                          
+      a1 <- tt;                                                                                                                 
+      b <- t0;                                                                                                                  
+      t00 <- VPSLL_8u32 b (W128.of_int 16);                                                                                     
+      r00 <- VPBLENDW_256 a1 t00 (W8.of_int 170);                                                                               
+      t10 <- VPSRL_8u32 a1 (W128.of_int 16);                                                                                    
+      r1 <- VPBLENDW_256 t10 b (W8.of_int 170);                                                                                 
+      (ttt, t0) <- (r00, r1);                                                                                                   
+      a2 <- t1;                                                                                                                 
+      b0 <- t2;                                                                                                                 
+      t01 <- VPSLL_8u32 b0 (W128.of_int 16);                                                                                    
+      r01 <- VPBLENDW_256 a2 t01 (W8.of_int 170);                                                                               
+      t11 <- VPSRL_8u32 a2 (W128.of_int 16);                                                                                    
+      r10 <- VPBLENDW_256 t11 b0 (W8.of_int 170);                                                                               
+      (tt, t2) <- (r01, r10);                                                                                                   
+      a3 <- t3;                                                                                                                 
+      b1 <- t4;                                                                                                                
+      t02 <- VPSLL_8u32 b1 (W128.of_int 16);                                                                                    
+      r02 <- VPBLENDW_256 a3 t02 (W8.of_int 170);                                                                               
+      t12 <- VPSRL_8u32 a3 (W128.of_int 16);                                                                                    
+      r11 <- VPBLENDW_256 t12 b1 (W8.of_int 170);                                                                               
+      (t1, t4) <- (r02, r11);                                                                                                   
+      a4 <- ttt;                                                                                                               
+      b2 <- tt;                                                                                                                 
+      t03 <- VMOVSLDUP_256 b2;                                                                                                  
+      t03 <- VPBLENDD_256 a4 t03 (W8.of_int 170);                                                                               
+      a4 <- VPSRL_4u64 a4 (W128.of_int 32);                                                                                     
+      t13 <- VPBLENDD_256 a4 b2 (W8.of_int 170);                                                                                
+      (t3, tt) <- (t03, t13);                                                                                                   
+      a5 <- t1;                                                                                                                 
+      b3 <- t0;                                                                                                                 
+      t04 <- VMOVSLDUP_256 b3;                                                                                                  
+      t04 <- VPBLENDD_256 a5 t04 (W8.of_int 170);                                                                               
+      a5 <- VPSRL_4u64 a5 (W128.of_int 32);                                                                                     
+      t14 <- VPBLENDD_256 a5 b3 (W8.of_int 170);                                                                                
+      (ttt, t0) <- (t04, t14);                                                                                                  
+      a6 <- t2;                                                                                                                 
+      b4 <- t4;                                                                                                                 
+      t05 <- VMOVSLDUP_256 b4;                                                                                                  
+      t05 <- VPBLENDD_256 a6 t05 (W8.of_int 170);                                                                               
+      a6 <- VPSRL_4u64 a6 (W128.of_int 32);                                                                                     
+      t15 <- VPBLENDD_256 a6 b4 (W8.of_int 170);                                                                                
+      (t1, t4) <- (t05, t15);                                                                                                   
+      a7 <- t3;                                                                                                                 
+      b5 <- ttt;                                                                                                                
+      r03 <- VPUNPCKL_4u64 a7 b5;                                                                                               
+      r12 <- VPUNPCKH_4u64 a7 b5;                                                                                               
+      (t2, ttt) <- (r03, r12);                                                                                                  
+      a8 <- t1;                                                                                                                 
+      b6 <- tt;                                                                                                                 
+      r04 <- VPUNPCKL_4u64 a8 b6;                                                                                               
+      r13 <- VPUNPCKH_4u64 a8 b6;                                                                                               
+      (t3, tt) <- (r04, r13);                                                                                                   
+      a9 <- t0;                                                                                                                 
+      b7 <- t4;                                                                                                                 
+      r05 <- VPUNPCKL_4u64 a9 b7;                                                                                               
+      r14 <- VPUNPCKH_4u64 a9 b7;                                                                                               
+      (t1, t4) <- (r05, r14);                                                                                                   
+      a10 <- t2;                                                                                                                
+      b8 <- t3;                                                                                                                 
+      r06 <- VPERM2I128 a10 b8 (W8.of_int 32);                                                                                  
+      r15 <- VPERM2I128 a10 b8 (W8.of_int 49);                                                                                  
+      (t0, t3) <- (r06, r15);                                                                                                   
+      a11 <- t1;                                                                                                                
+      b9 <- ttt;                                                                                                                
+      r07 <- VPERM2I128 a11 b9 (W8.of_int 32) ;                                                                                 
+      r16 <- VPERM2I128 a11 b9 (W8.of_int 49) ;                                                                                 
+      (t2, ttt) <- (r07, r16);                                                                                                  
+      a12 <- tt;                                                                                                                
+      b10 <- t4;                                                                                                                
+      r08 <- VPERM2I128 a12 b10 (W8.of_int 32);                                                                                 
+      r17 <- VPERM2I128 a12 b10 (W8.of_int 49);                                                                                 
+      (t1, t4) <- (r08, r17);                                                                                                   
+      rp <-                                                                                                                    
+        Array384.init                                                                                                          
+          (WArray384.get8                                                                                            
+             (WArray384.set256_direct (WArray384.init8 (fun (i_0 : int) => rp.[i_0])) (192 * i0) t0));      
+      rp <-                                                                                                                    
+        Array384.init                                                                                                          
+          (WArray384.get8                                                                                            
+             (WArray384.set256_direct (WArray384.init8 (fun (i_0 : int) => rp.[i_0])) (192 * i0 + 32) t2)); 
+      rp <-                                                                                                                    
+        Array384.init                                                                                                          
+          (WArray384.get8                                                                                            
+             (WArray384.set256_direct (WArray384.init8 (fun (i_0 : int) => rp.[i_0])) (192 * i0 + 64) t1)); 
+      rp <-                                                                                                                    
+        Array384.init                                                                                                          
+          (WArray384.get8                                                                                            
+             (WArray384.set256_direct (WArray384.init8 (fun (i_0 : int) => rp.[i_0])) (192 * i0 + 96) t3)); 
+      rp <-                                                                                                                    
+        Array384.init                                                                                                          
+          (WArray384.get8                                                                                            
+             (WArray384.set256_direct (WArray384.init8 (fun (i_0 : int) => rp.[i_0])) (                    
+                192 * i0 + 128) ttt));                                                                                          
+      rp <-                                                                                                                    
+        Array384.init                                                                                                          
+          (WArray384.get8                                                                                            
+             (WArray384.set256_direct (WArray384.init8 (fun (i_0 : int) => rp.[i_0])) (192 * i0 + 160) t4));
+      i0 <- i0 + 1;                                                                                                             
+    }                                                                                                                          
+    (aux, aux_0) <- (rp, a0);                                                                                                   
+    r <- Array1152.init (fun (i_0 : int) => if 384 * i <= i_0 < 384 * i + 384 then aux.[i_0 - 384 * i] else r.[i_0]);           
+    a <- Array768.init (fun (i_0 : int) => if 256 * i <= i_0 < 256 * i + 256 then aux_0.[i_0 - 256 * i] else a.[i_0]);         
+    i <- i + 1;                                                                                                                 
+  }
+  return r;
+ }       
+}.
+
+op nttpack_16 (rp : W16.t Array256.t)  = init_256_16 (fun (i : int) => rp.[nttpack_idx.[i]]).
+
+op nttpackv_16 (v : W16.t Array768.t) =
+  init_768_16
+    (fun (i : int) =>
+       if 0 <= i < 256 then (nttpack_16 (subarray256 v 0)).[i]
+       else
+         if 256 <= i < 512 then (nttpack_16 (subarray256 v 1)).[i - 256]
+         else  (nttpack_16 (subarray256 v 2)).[i - 512]).
+
+lemma nttpackv_16E v : nttpackv_16 v = nttpackv v.
+rewrite /nttpackv_16 /init_768_16 /nttpack_16 /init_256_16.
+by rewrite /nttpackv /nttpack.
+qed.
+
+
+
+lemma auxtobytes_corr_h (_aw : W16.t Array768.t):
+    hoare[AuxToBytes.__i_polyvec_tobytes :
+             pos_bound768_cxq a 0 768 2 /\ a = _aw ==> 
+    res = Array1152.of_list W8.zero (ByteEncode 12 (to_list (map asint (lift_array768 (nttpackv _aw)))))]. 
+proc;inline *.
+proc change ^while.1: {rp <- init_384_8 (fun i_0 => r.[384 * i + i_0]);};1: by auto.
+proc change ^while.2: {a0 <- init_256_16 (fun i_0 => a.[256 * i + i_0]);};1: by auto.
+(* FIXME: CHECK qx16 initialization inside while *)
+proc change ^while.4: {qx16 <- sliceget16_16_256 jqx16 0;}; 1: by auto.
+proc change ^while.^while.1: { r0 <- sliceget256_16_256 rp0 (i1*256);}; 1: by auto => /#.
+proc change ^while.^while.9 : {rp0 <- sliceset256_16_256 rp0 (i1*256) r0;}; 1: by auto => /> /#.
+proc change ^while.^while{2}.1 : {t0 <- sliceget256_16_256 a0 (8*i0*256);};1: by auto => /#.
+proc change ^while.^while{2}.2 : {t1 <- sliceget256_16_256 a0 ((8*i0+1)*256);};1: by auto => /#.
+proc change ^while.^while{2}.3 : {t2 <- sliceget256_16_256 a0 ((8*i0+2)*256);};1: by auto => /#.
+proc change ^while.^while{2}.4 : {t3 <- sliceget256_16_256 a0 ((8*i0+3)*256);};1: by auto => /#.
+proc change ^while.^while{2}.5 : {t4 <- sliceget256_16_256 a0 ((8*i0+4)*256);};1: by auto => /#.
+proc change ^while.^while{2}.6 : {t5 <- sliceget256_16_256 a0 ((8*i0+5)*256);};1: by auto => /#.
+proc change ^while.^while{2}.7 : {t6 <- sliceget256_16_256 a0 ((8*i0+6)*256);};1: by auto => /#.
+proc change ^while.^while{2}.8 : {t7 <- sliceget256_16_256 a0 ((8*i0+7)*256);};1: by auto => /#.
+proc change ^while.^while{2}.105 : {rp <- sliceset384_8_256 rp (192*i0*8) t0;};1: by auto => /#.
+proc change ^while.^while{2}.106 : {rp <- sliceset384_8_256 rp ((192*i0+32)*8) t2;};1: by auto => /#.
+proc change ^while.^while{2}.107 : {rp <- sliceset384_8_256 rp ((192*i0+64)*8) t1;};1: by auto => /#.
+proc change ^while.^while{2}.108 : {rp <- sliceset384_8_256 rp ((192*i0+96)*8) t3;};1: by auto => /#.
+proc change ^while.^while{2}.109 : {rp <- sliceset384_8_256 rp ((192*i0+128)*8) ttt;};1: by auto => /#.
+proc change ^while.^while{2}.110 : {rp <- sliceset384_8_256 rp ((192*i0+160)*8) t4;};1: by auto => /#.
+proc change ^while.11: { r <- init_1152_8 (fun (i_0 : int) => if 384 * i <= i_0 < 384 * i + 384 then aux.[i_0 - 384 * i] else r.[i_0]);}; 1: by auto.
+proc change ^while.12: { a <- init_768_16  (fun (i_0 : int) => if 256 * i <= i_0 < 256 * i + 256 then aux_0.[i_0 - 256 * i] else a.[i_0]);};1: by auto. 
+
+unroll for ^while.
+do 6!(unroll for ^while).
+cfold ^i<-.
+cfold ^i0<-.
+cfold ^i1<-.
+wp -3.
+
+
+conseq (: 
+ a = _aw /\
+   Array768.all (fun bv => W16.zero \sle bv /\ bv \slt (of_int (2 * 3329))) a
+   ==> r =  let ret = init_768_12 (fun j => tobytes_circuit (nttpackv_16 _aw).[j]) in
+  init_1152_8 (fun i =>
+    W8.init (fun j =>
+      let idx = i*8 + j in
+      let aidx = idx %/ 12 in
+      let bidx = idx %% 12 in
+      W12."_.[_]" (ret.[aidx]) bidx))); last by circuit.
+      
++ move => &hr />; rewrite allP /= /pos_bound768_cxq /(\sle) /(\slt) /= /qE /smod /=.
+  by rewrite qE /= => H k ?; move : (H k _) => //=.
+
+move => &hr [#]/=; rewrite /pos_bound768_cxq /bpos16 => H0 <- rr ->.
+rewrite /init_1152_8 /encode12 tP => i ib.
+rewrite initiE 1:/# /= get_of_list 1:/# /= wordP => k kb.
+rewrite initiE //= /init_256_12 initiE 1:/# /=.
+have := nttpackv_pred a{hr} (fun c => bpos16 c (2 * q)).
+rewrite !allP  /= iffE qE /= => [#_ H].
+by rewrite nttpackv_16E  to_bytes_circuit_sem_polyvec;1..3:
+ by rewrite /(\ult) /=; smt(W16.to_sint_unsigned).
+ qed.
+
+
+lemma auxtobytes_ll : islossless AuxToBytes.__i_polyvec_tobytes.
+proc.
+inline *. 
+do 7!(unroll for ^while); auto. 
+qed.
+
+lemma auxtobytes_corr (_aw : W16.t Array768.t):
+    phoare[ AuxToBytes.__i_polyvec_tobytes :
+             pos_bound768_cxq a 0 768 2 /\ a = _aw ==> 
+    res = Array1152.of_list W8.zero (ByteEncode 12 (to_list (map asint (lift_array768 (nttpackv _aw)))))] = 1%r
+  by conseq auxtobytes_ll (auxtobytes_corr_h _aw).
+
+
+lemma polyvec_tobytes_corr (_aw : W16.t Array768.t):
+    phoare[ Jkem_avx2.M.__i_polyvec_tobytes :
+             pos_bound768_cxq a 0 768 2 /\ a = _aw ==> 
+    res = Array1152.of_list W8.zero (ByteEncode 12 (to_list (map asint (lift_array768 (nttpackv _aw)))))] = 1%r.
+proof.
+bypr => &m [??].
+have <- : Pr[AuxToBytes.__i_polyvec_tobytes(r{m}, _aw) @ &m : res = Array1152.of_list W8.zero (ByteEncode 12 (to_list (map asint (lift_array768 (nttpackv _aw)))))] = 1%r
+ by byphoare (auxtobytes_corr _aw)  =>/=; 1:smt().
+byequiv (: ={arg} /\ a{1} = _aw /\
+             pos_bound768_cxq a{1} 0 768 2 ==> ={res}) => //.
+proc => /=. 
+inline M._i_poly_tobytes.
+while (={r, a,i} /\ 0 <= i{1} <= 4 /\
+   pos_bound768_cxq a{1} 0 768 2); last by auto => /> /#.
+seq 3 3 : (#pre /\ ={rp,a0} /\
+   pos_bound256_cxq a0{1} 0 256 1).
++ ecall {1} (poly_csubq_avx2_corr a0{1}).
+  ecall {2} (poly_csubq_avx2_corr a0{2}).
+  auto => /> &1; rewrite /pos_bound768_cxq /pos_bound256_cxq /lift_array256 /= qE /= => ????;split; 1: by smt(Array256.initiE).
+  move => ? rr1.
+  rewrite !tP;move =>  Hrr11 Hrr12 rr2.
+  rewrite !tP;move =>  Hrr21 Hrr22.
+  move => ii iib. 
+  have := Hrr11 ii iib; rewrite !mapiE 1,2:/# /=. 
+  have := Hrr12 ii iib.  
+  have := Hrr21 ii iib; rewrite !mapiE 1,2:/# /=. 
+  have := Hrr22 ii iib.  
+  rewrite /to_sint /smod /=. 
+  move => Hrr11i Hrr12i Hrr21i Hrr22i.
+  have Hn1 : !(32768 <= to_uint rr2.[ii]) by smt(W16.to_uint_cmp pow2_16).
+  have Hn2 : !(32768 <= to_uint rr1.[ii]) by smt(W16.to_uint_cmp pow2_16).
+  have Hn3 : !(32768 <= to_uint _aw.[ii]) by smt(W16.to_uint_cmp pow2_16).
+  move : Hrr11i Hrr12i Hrr21i Hrr22i; rewrite Hn1 Hn2 /=.
+  move => Hrr11i Hrr12i Hrr21i Hrr22i.
+  move : Hrr12i; rewrite -Hrr22i -eq_incoeff.  
+  by rewrite !modz_small ?qE /= 1,2:/# to_uint_eq /#.
+
+wp;while (#pre /\ ={i0} /\ 0<=i0{1}<=2); last first.
++ auto => /> &2 ?????i0r????;split;1:smt().
+  rewrite /pos_bound768_cxq => k kb; rewrite initiE 1:/# /= /#.
+
+wp -1 -1; conseq (: _ ==> ={rp}); 1: by smt().
+
+inline *;sim; auto => /> &1 &2 ???;rewrite /pos_bound256_cxq qE /= => Hb ???.
+
+have Hpos : forall jj kk ii, 0 <= jj < 8 => 0 <= kk < 16 => 0 <= ii < 16 => (get256 (WArray512.init16 ("_.[_]" a0{1})) (8 * i0{1} + jj) \bits16 kk).[ii] = a0{1}.[kk + 16*jj + i0{1}*128].[ii] by
+  move => jj kk ii jjb kkb iib; rewrite get256E /pack32_t /(\bits16) initiE 1:/# /= initiE 1:/# /= initiE 1:/# /= initiE 1:/# /= /(\bits8) initiE 1:/# /= /#.
+
+have bits : forall kk ii, 0 <= kk < 256 => 12 <= ii < 16 => !a0{1}.[kk].[ii].
++ move => kk ii kkb iib; have := Hb kk kkb;rewrite /to_sint /smod /= => Hn.
+  have Hn1 : !32768 <= to_uint a0{1}.[kk] by smt(W16.to_uint_cmp pow2_16).
+  move : Hn; rewrite Hn1 /= get_to_uint . 
+  have ? : 4096 <= 2^ii;last by smt().
+  have ? : 4096 = 2^12 by auto.
+  smt(@StdOrder.IntOrder). 
+
+have bitsC : forall  ii, 0 <= ii < 16 => (W16.of_int 4095).[ii] <=> 0<=ii<12.
++ move => ii iib.
+  have : all (fun i => (W16.of_int 4095).[i] <=> 0 <= i < 12) (iota_ 0 16); 
+  last by rewrite allP => H; move : (H ii _);smt(mem_iota).
+  by rewrite -iotaredE /= !get_to_uint /=.
+
+
+do split; rewrite /VPBROADCAST_16u16 /= -(W16u16.unpack16K (WArray512.get256 _ _)) -(W16u16.unpack16K (W16u16.pack16 _)) !andb16u16E;congr;rewrite packP => k kb;rewrite map2iE 1:/# /= andE wordP => ii iib;rewrite map2iE 1:/# /= get_of_list 1:/# /= (nth_map witness)  /=;1,3,5,7,9,11,13,15:smt(size_iota); rewrite unpack16E initiE 1:/# /=;1..7: by rewrite Hpos /#.
+      have /= -> := Hpos 0;smt().
+qed.
+
+
+lemma signed_bound768_cxq_small r (i j:int) :
+  i <= j => signed_bound768_cxq r 0 768 i => signed_bound768_cxq r 0 768 j.
+rewrite /signed_bound768_cxq => />Hij H k Hk1 Hk2. move :(H k). rewrite Hk1 Hk2 => />. smt(). qed.
+
