proof/correctness/avx2/common/MLKEM_Poly_avx2_circuit.ec
@@ -1,0 +1,213 @@
+require import AllCore List Int IntDiv CoreMap Real Number Ring StdOrder BitEncoding.
+
+from Jasmin require import JModel.
+from JazzEC require import Array400 Array384 Array256 Array128 Array64 Array32 Array16 Array8 Array4 Array2.
+from JazzEC require import WArray512 WArray128 WArray384 WArray32 WArray16.
+from JazzEC require import Jkem_avx2.
+
+require import AVX2_Ops W16extra.
+require import Fq NTT_Fq MLKEMFCLib.
+require import Fq_avx2 NTT_avx2_poly.
+require import MLKEM_Poly_avx2.
+require import Mlkem_bindings.
+require import Circuit_semantics.
+from Spec require import GFq Rq Serialization VecMat Sampling EncDecCorrectness Correctness.
+
+import BitChunking BS2Int.
+import Fq.
+import GFq Rq Serialization VecMat.
+import Zq ZModP.
+import Fq_avx2.
+import MLKEM_PolyAVX.
+
+
+lemma poly_csubq_avx2_ll :
+   islossless Jkem_avx2.M._poly_csubq.
+by proc;inline *;unroll for ^while;auto.
+qed.
+
+lemma poly_csubq_avx2_corr_h (_aw : W16.t Array256.t):
+    hoare[ Jkem_avx2.M._poly_csubq  :
+             rp = _aw /\
+             pos_bound256_cxq rp 0 256 2 ==> 
+             lift_array256 res = lift_array256 _aw /\
+             pos_bound256_cxq res 0 256 1]. 
+proof.
+proc; inline *.
+proc change 1: { qx16 <- sliceget16_16_256 jqx16 0;}; 1: by auto.
+proc change ^while.1: { r <- sliceget256_16_256 rp (i*256);};1: by auto => /#.
+proc change ^while.9: { rp <-sliceset256_16_256 rp (i*256) r;};1: by auto => /#.
+unroll for ^while.
+cfold ^i<-.
+wp -1.
+conseq (: rp = _aw /\ all (fun c => W16.zero \sle c && c \slt W16.of_int 6658) rp ==>
+       rp = init_256_16 (fun i => csubq_circuit _aw.[i])); last by circuit.
+
+       
+(* BDEP pre conseq *)
++ move => &hr />. rewrite /pos_bound256_cxq /bpos16 qE /= => H.
+  rewrite /(\slt) /(\sle) /= /smod /= allP /=.
+  by exact H.
+
+(* BDEP post conseq *)
+
+(* We start with some boilerplate *)
+move => &hr [#]/= ->; rewrite /pos_bound256_cxq => Hb rr; rewrite /init_256_16 /lift_array256 /= => ->; split.
+
+rewrite tP => i ib.
+rewrite !mapiE 1,2:/# /= initiE 1:/# /=.
+rewrite /csubq_circuit ultE /W16_sub /=.
+move : (Hb i ib);rewrite /bpos16 qE /= /to_sint /smod /=.
+case (to_uint _aw.[i] < 3329) => *//;1:
+have ->/= : !32768 <= to_uint _aw.[i] by smt(W16.to_uint_cmp).
+rewrite to_uintB /=;1: by rewrite uleE => /#.
+have ->/= : !32768 <= to_uint _aw.[i] - 3329;  by smt(W16.to_uint_cmp).
+
+move => i ib.
+rewrite initiE 1:/# /= /csubq_circuit ultE /W16_sub /=.
+move : (Hb i ib);rewrite /bpos16 qE /= /to_sint /smod /=.
+case (to_uint _aw.[i] < 3329) => *//;1:
+have ->/= : !32768 <= to_uint _aw.[i] by smt(W16.to_uint_cmp).
+by smt(W16.to_uint_cmp).
+rewrite to_uintB /=;1: by rewrite uleE => /#.
+have ->/= : !32768 <= to_uint _aw.[i] - 3329;  by smt(W16.to_uint_cmp).
+qed.
+
+lemma poly_csubq_avx2_corr (_aw : W16.t Array256.t):
+    phoare[ Jkem_avx2.M._poly_csubq  :
+             rp = _aw /\
+             pos_bound256_cxq rp 0 256 2 ==> 
+             lift_array256 res = lift_array256 _aw /\
+             pos_bound256_cxq res 0 256 1] = 1%r
+  by conseq poly_csubq_avx2_ll (poly_csubq_avx2_corr_h _aw).
+
+
+lemma poly_add_corr_avx_impl ab bb :
+    0 <= ab <= 6 => 0 <= bb <= 3 => 
+  forall _a _b,
+      phoare[ Mprevec.poly_add2 :
+           _a = lift_array256 rp /\
+           _b = lift_array256 bp /\
+           signed_bound_cxq rp 0 256 ab /\
+           signed_bound_cxq bp 0 256 bb 
+           ==>
+           signed_bound_cxq res 0 256 (ab + bb) /\ 
+           forall k, 0 <= k < 256 =>
+              incoeff (to_sint res.[k]) = _a.[k] + _b.[k]] = 1%r
+   by move => abb bbb _a _b; apply (MLKEM_PolyAVX.poly_add_corr _a _b ab bb abb bbb).
+
+lemma poly_frommsg_ll : islossless Jkem_avx2.M._i_poly_frommsg 
+ by proc; inline *;wp;while (0 <= i <= 32) (32-i);  by  auto =>  /> /#.
+
+lemma poly_frommsg_corr_h (_m : W8.t Array32.t): 
+    hoare [Jkem_avx2.M._i_poly_frommsg :
+             ap =  _m 
+              ==>
+             lift_array256 res = decompress_poly 1 (decode1 _m) /\
+             pos_bound256_cxq res 0 256 1 ].
+proc; inline *.
+proc change 1: { hqs <- sliceget16_16_256 hqx16_p1 0;};1: by auto.
+proc change 2: { shift <- VPBROADCAST_2u128 (sliceget4_32_128 pfm_shift_s 0);};1: by auto.
+proc change 3: { idx <- VPBROADCAST_2u128 (sliceget16_8_128 pfm_idx_s 0);};1: by auto.
+proc change 4: { f <- sliceget32_8_256 ap 0;};1: by auto.
+proc change ^while.23 : { rp <- sliceset256_16_256 rp (2*i*256) g0;}; 1: by auto => /#. 
+proc change ^while.24 : { rp <- sliceset256_16_256 rp ((2*i+1)*256) g1;}; 1: by auto => /#. 
+proc change ^while.25 : { rp <- sliceset256_16_256 rp ((2*i+8)*256) g2;}; 1: by auto => /#. 
+proc change ^while.26 : { rp <- sliceset256_16_256 rp ((2*i+9)*256) g3;}; 1: by auto => /#. 
+
+
+unroll for ^while.
+wp -1.
+
+
+conseq (: _ ==> rp = init_256_16 (fun i => decompress1_circuit _m.[i %/ 8].[i %% 8]));
+ 2: by circuit.
+
+(* BDEP post conseq *)
+
+move => &hr [#]/= <- rr /= ->.
+
+split.
++ rewrite tP => i ib.
+  rewrite /init_256_16 !mapiE 1,2:/# /= -get_to_list /= initiE 1:/# /=.
+  by rewrite /decompress1_circuit decompress1_circuit_sem //.
+
+rewrite /pos_bound256_cxq qE /= => k kb. 
+rewrite /init_256_16 initiE 1:/# /=.
+by smt(decompress1_circuit_rng).
+qed.
+
+
+(********** END BDEP PROOF OF FROMMSG **************)
+
+
+lemma poly_frommsg_corr (_m : W8.t Array32.t): 
+    phoare [Jkem_avx2.M._i_poly_frommsg :
+             ap =  _m 
+              ==>
+             lift_array256 res = decompress_poly 1 (decode1 _m) /\
+             pos_bound256_cxq res 0 256 1 ] = 1%r
+  by conseq poly_frommsg_ll (poly_frommsg_corr_h _m).
+
+lemma poly_tomsg_ll : islossless Jkem_avx2.M._i_poly_tomsg.
+proc.
+cfold 7.
+inline *.
+do 2!(unroll for ^while).
+auto.
+qed.
+
+(********** BEGIN BDEP PROOF OF TOMSG **************)
+
+
+lemma poly_tomsg_corr_h _aw : 
+    hoare [Jkem_avx2.M._i_poly_tomsg :
+             pos_bound256_cxq a 0 256 2 /\ 
+              a = _aw
+              ==>
+             res.`1 = encode1 (compress_poly 1 (lift_array256 _aw))  ].
+proof.
+proc; inline *.
+proc change 3 : { qx16 <- sliceget16_16_256 jqx16 0;};1: by auto.
+proc change ^while.1: { r <- sliceget256_16_256 rp0 (i0*256);};1: by auto => /#.
+proc change ^while.9: { rp0 <- sliceset256_16_256 rp0 (i0*256) r;};1: by auto => /#.
+proc change 8: {hq <- sliceget16_16_256 px16 0;}; 1: by auto.
+proc change 10: {hhq <- sliceget16_16_256 px16 0;}; 1: by auto.
+proc change ^while{2}.1: { f0 <- sliceget256_16_256 a (2*i*256);};1: by auto => /#.
+proc change ^while{2}.2: { f1 <- sliceget256_16_256 a ((2*i+1)*256);};1: by auto => /#.
+proc change ^while{2}.14 : { rp <- sliceset32_8_32 rp  (i*32) c;};1: by auto => /#.
+
+
+cfold 11.
+unroll for ^while.
+cfold ^i0<-.
+unroll for ^while.
+wp -3. 
+
+
+conseq (: a = _aw /\
+   Array256.all (fun bv => W16.zero \sle bv /\ bv \sle (of_int (2 * 3329))) a ==> rp = init_32_8 (fun i => W8.init (fun j => compress1_circuit _aw.[i*8+j]))); last  by circuit.
+
+(* conseq pre *)
++ move => &hr />; rewrite /pos_bound256_cxq qE /= /(\sle) allP /=  => Hb i ib /=.
+  rewrite /(to_sint W16.zero) /= /(W16.smod 0) /=.
+  rewrite /(to_sint (W16.of_int 6658)) /= /(W16.smod 6658) /= /#.
+
+(* BDEP post conseq *)
+move => &hr [#]/= H0 <- rr ->; rewrite /= /init_32_8 tP => i ib.
+rewrite wordP => k kb; rewrite !initiE 1..3:/# /=.
+rewrite encode_compress_bits //=.
+by apply compress1_circuit_sem.
+qed.
+
+
+(********** END BDEP PROOF OF TOMSG **************)
+
+
+lemma poly_tomsg_corr _aw : 
+    phoare [Jkem_avx2.M._i_poly_tomsg :
+             pos_bound256_cxq a 0 256 2 /\ 
+              a = _aw
+              ==>
+             res.`1 = encode1 (compress_poly 1 (lift_array256 _aw))  ] = 1%r
+  by conseq poly_tomsg_ll (poly_tomsg_corr_h _aw).
